InstantiationProp.v
@@ -1,756 +1,326 @@
-From stdpp Require Import mapset fin_maps.
-From CT Require Import CoreLangProp.
+From stdpp Require Import mapset.
+From CT Require Import Syntax.
 From CT Require Import OperationalSemantics.
-From CT Require Import BasicTypingProp.
-From CT Require Import Qualifier.
-From CT Require Import RefinementTypeProp.
-From CT Require Import Denotation.
-From CT Require Import Instantiation.
+From CT Require Import BasicTypingProp Lc Denotation Typing.
 
-Import Atom.
-Import CoreLang.
-Import Tactics.
-Import NamelessTactics.
-Import OperationalSemantics.
-Import BasicTyping.
-Import ListCtx.
-Import Qualifier.
-Import Denotation.
-Import RefinementType.
+Import BaseDef MyTactics Primitives Lang LangLc Qualifier OperationalSemantics BasicTyping BasicTypingProp Instantiation RtyLc Lc Denotation ListCtx Typing InstantiationLc.
 
-(** This file proves auxiliary lemmas about multi-substitution and provides
-  handy tactics. *)
-
-Lemma closed_env_insert env x v :
-  env !! x = None ->
-  closed_env (<[x:=v]>env) ->
-  closed_value v /\ closed_env env.
+Class MsubstPreservesClosed A `{Stale A} `{Subst value A} := msubst_preserves_closed :
+forall Γ Γ' (ρ: A) (σ: env),
+  ctxEnv Γ σ ->
+  stale ρ ⊆ stale (Γ ++ Γ') ->
+  stale (m{σ} ρ) ⊆ stale (Γ').
+  
+Lemma MsubstPreservesClosed_all
+(A : Type)
+(staleA : Stale A)
+(substA : Subst value A)
+(fv_of_msubst_closedA : @FvOfMsubstClosed A staleA substA)
+: @MsubstPreservesClosed A staleA substA.
 Proof.
-  intro.
-  unfold closed_env.
-  rewrite map_Forall_insert; eauto.
+  unfold MsubstPreservesClosed.
+  intros Γ Γ' ρ σ HΓ Hρ.
+  rewrite fv_of_msubst_closedA by eauto using ctxEnv_closed_env.
+  ln_simpl.
+  apply ctxEnv_dom in HΓ. rewrite HΓ in *.
+  my_set_solver.
 Qed.
 
-Ltac apply_msubst_ind :=
-  unfold msubst;
-  match goal with
-  | |- ?T =>
-      match T with
-      | context [map_fold ?a ?b ?m] =>
-          match eval pattern (map_fold a b m) in T with
-          | ?P _ =>
-              match eval pattern m in P with
-              | ?P _ =>
-                  (* let P := eval simpl in (fun r m => P m r) in *)
-                  let P := eval simpl in (fun m => P m (msubst a m b)) in
-                    apply (fin_maps.map_fold_ind P); unfold msubst
-              end
-          end
-      end
-  end.
-
-Ltac gen_closed_env :=
-  repeat
-    match goal with
-    | H : closed_env (<[?i:=_]> ?m), H' : ?m !! ?i = None |- _ =>
-        let H1 := fresh "H" in
-        let H2 := fresh "H" in
-        destruct (closed_env_insert _ _ _ H' H) as [H1 H2];
-        uniq_hyp H1; uniq_hyp H2
-    | H : closed_env ?m, H' : ?m !! _ = Some ?v |- _ =>
-        let T := fresh "H" in
-        assert (closed_value v) as T by eauto;
-        uniq_hyp T
-    end.
-
-Lemma msubst_insert {T: Type}
-  (f_subst: atom -> value -> T -> T)
-  (subst_commute: forall x u_x y u_y e,
-      x <> y -> x ∉ fv_value u_y -> y ∉ fv_value u_x ->
-      f_subst x u_x (f_subst y u_y e) =
-        f_subst y u_y (f_subst x u_x e))
-  :
-  forall (Γv: env) (x: atom) (v_x: value) (e: T),
-    closed_env Γv ->
-    closed_value v_x ->
-    Γv !! x = None ->
-    msubst f_subst (<[x:=v_x]> Γv) e = f_subst x v_x (msubst f_subst Γv e).
+#[global] Instance MsubstPreservesClosed_tm: MsubstPreservesClosed tm.
 Proof.
-  intros.
-  apply map_fold_insert_L; eauto.
-  intros.
-  assert (closed_env (<[x:=v_x]>Γv)). {
-    apply map_Forall_insert; eauto.
-  }
-  gen_closed_env.
-  apply subst_commute; eauto; my_set_solver.
+  eapply MsubstPreservesClosed_all; typeclasses eauto.
 Qed.
 
-Ltac fold_forward :=
-  repeat match goal with
-    | H : map_fold ?f ?x ?m = _ |- context [ map_fold ?f ?x ?m ] => setoid_rewrite H
-    | H : forall _ _ _ _, map_fold _ _ (<[?i:= _]> _) = _ ?i _ (map_fold _ _ _) |-
-                       context [map_fold _ _ (<[?i:= _]> _) ] =>
-        rewrite H
-    | H : forall _ _ _ _, map_fold _ _ (<[?i:= _]> _) = _ ?i _ (map_fold _ _ _), H': context [map_fold _ _ (<[?i:= _]> _) ] |- _ =>
-        rewrite H in H'
-    end; eauto.
-
-Ltac msubst_tac :=
-  intros *; apply_msubst_ind; intros; subst; simpl; eauto;
-  gen_closed_env; simp_hyps; subst; fold_forward.
-
-Ltac fold_msubst := change (map_fold ?s ?e ?m) with (msubst s m e) in *.
-
-Ltac rewrite_msubst_insert :=
-  cbn; fold_msubst; rewrite !msubst_insert;
-  eauto using subst_commute_value, subst_commute_tm, subst_commute_qualifier,
-    subst_commute_rty.
-
-Lemma rty_erase_msubst_eq ρ Γv :
-  rty_erase ρ = rty_erase (m{Γv}r ρ).
+#[global] Instance MsubstPreservesClosed_value: MsubstPreservesClosed value.
 Proof.
-  msubst_tac.
-  qauto using rty_erase_subst_eq.
+  eapply MsubstPreservesClosed_all; typeclasses eauto.
 Qed.
 
-Ltac msubst_hyp_rewrite :=
-  match goal with
-  | H : (msubst ?f ?m ?x) = _ |-
-      context [(msubst ?f ?m ?x) ] =>
-      rewrite H
-  end.
-
-Lemma msubst_qualifier: forall Γv ϕ,
-    closed_env Γv ->
-    (m{Γv}q) ϕ =
-      match ϕ with
-      | qual vals prop =>
-          qual (vmap (m{Γv}v) vals) prop
-      end.
+#[global] Instance MsubstPreservesClosed_qualifier: MsubstPreservesClosed qualifier.
 Proof.
-  msubst_tac.
-  - destruct ϕ. erewrite Vector.map_ext.
-    by rewrite Vector.map_id.
-    intros. simpl.
-    by rewrite map_fold_empty.
-  - destruct ϕ.
-    simpl.
-    f_equal. rewrite Vector.map_map.
-    apply Vector.map_ext.
-    intros; rewrite_msubst_insert.
+  eapply MsubstPreservesClosed_all; typeclasses eauto.
 Qed.
 
-Lemma msubst_qualifier_and Γv q1 q2 :
-  closed_env Γv ->
-  m{Γv}q (q1 & q2) = (m{Γv}q q1) & (m{Γv}q q2).
+#[global] Instance MsubstPreservesClosed_rty: MsubstPreservesClosed rty.
 Proof.
-  msubst_tac. apply qualifier_and_subst.
+  eapply MsubstPreservesClosed_all; typeclasses eauto.
 Qed.
 
-Lemma msubst_constant: forall Γv (c: constant), (m{Γv}v) c = c.
+Class MsubstPreservesClosedEmpty A `{Stale A} `{Subst value A} := msubst_preserves_closed_empty :
+forall Γ (ρ: A) (σ: env),
+  ctxEnv Γ σ ->
+  stale ρ ⊆ stale Γ ->
+  stale (m{σ} ρ) = ∅.
+  
+Lemma MsubstPreservesClosedEmpty_all
+(A : Type)
+(staleA : Stale A)
+(substA : Subst value A)
+(msubst_preserves_closedA : @MsubstPreservesClosed A staleA substA)
+: @MsubstPreservesClosedEmpty A staleA substA.
 Proof.
-  msubst_tac.
+  unfold MsubstPreservesClosedEmpty.
+  intros Γ ρ σ HΓ Hρ.
+  pose proof (msubst_preserves_closedA Γ [] ρ σ HΓ) as H; eauto.
+  listctx_set_simpl. ln_simpl. my_set_solver.
 Qed.
 
-Lemma msubst_bvar: forall Γv n, (m{Γv}v) (vbvar n) = vbvar n.
+#[global] Instance MsubstPreservesClosedEmpty_tm: MsubstPreservesClosedEmpty tm.
 Proof.
-  msubst_tac.
+  eapply MsubstPreservesClosedEmpty_all; typeclasses eauto.
 Qed.
 
-Lemma msubst_fvar: forall Γv (x : atom),
-    closed_env Γv ->
-    (m{Γv}v) x = match Γv !! x with
-                 | Some v => v
-                 | None => x
-                 end.
+#[global] Instance MsubstPreservesClosedEmpty_value: MsubstPreservesClosedEmpty value.
 Proof.
-  msubst_tac.
-  destruct (decide (x = i)); subst; simplify_map_eq. reflexivity.
-  case_match.
-  apply subst_fresh_value.
-  gen_closed_env. my_set_solver.
-  simpl. rewrite decide_False; eauto.
+  eapply MsubstPreservesClosedEmpty_all; typeclasses eauto.
 Qed.
 
-Lemma msubst_lam: forall Γv T e,
-    closed_env Γv ->
-    ((m{Γv}v) (vlam T e)) = (vlam T ((m{Γv}t) e)).
+#[global] Instance MsubstPreservesClosedEmpty_qualifier: MsubstPreservesClosedEmpty qualifier.
 Proof.
-  msubst_tac.
+  eapply MsubstPreservesClosedEmpty_all; typeclasses eauto.
 Qed.
 
-Lemma msubst_fix: forall Γv T e,
-    closed_env Γv ->
-    ((m{Γv}v) (vfix T e)) = (vfix T ((m{Γv}t) e)).
+#[global] Instance MsubstPreservesClosedEmpty_rty: MsubstPreservesClosedEmpty rty.
 Proof.
-  msubst_tac.
+  eapply MsubstPreservesClosedEmpty_all; typeclasses eauto.
 Qed.
 
-Lemma msubst_value: forall Γv (v:value),
-    closed_env Γv ->
-    (m{Γv}t) (treturn v) = (m{Γv}v) v.
-Proof.
-  msubst_tac.
-Qed.
-
-Lemma msubst_match: forall Γv (v: value) e1 e2,
-    closed_env Γv ->
-    ((m{Γv}t) (tmatchb v e1 e2)) = tmatchb (m{Γv}v v) (m{Γv}t e1) (m{Γv}t e2).
-Proof.
-  msubst_tac.
-Qed.
-
-Lemma msubst_lete: forall (Γv: env) e_x e,
-    closed_env Γv ->
-    (m{Γv}t (tlete e_x e) = tlete ((m{Γv}t) e_x) ((m{Γv}t) e)).
-Proof.
-  msubst_tac.
-Qed.
-
-Lemma msubst_tleteffop: forall Γv op (v2: value) e,
-    closed_env Γv ->
-    (m{Γv}t) (tleteffop op v2 e) = (tleteffop op (m{Γv}v v2) (m{Γv}t e)).
-Proof.
-  msubst_tac.
-Qed.
-
-Lemma msubst_tletapp: forall Γv (v1 v2: value) e,
-    closed_env Γv ->
-    (m{Γv}t) (tletapp v1 v2 e) = (tletapp (m{Γv}v v1) (m{Γv}v v2) (m{Γv}t e)).
-Proof.
-  msubst_tac.
-Qed.
-
-Lemma msubst_overrty: forall Γv b ϕ,
-    closed_env Γv ->
-    (m{Γv}r) {:b|ϕ} = {:b| (m{Γv}q) ϕ}.
-Proof.
-  msubst_tac.
-Qed.
-
-Lemma msubst_underrty: forall Γv b ϕ,
-    closed_env Γv ->
-    ((m{Γv}r) ([:b|ϕ])) = ([:b|(m{Γv}q) ϕ]).
-Proof.
-  msubst_tac.
-Qed.
-
-Lemma msubst_arrrty: forall Γv ρ τ,
-    closed_env Γv ->
-    ((m{Γv}r) (ρ⇨τ)) = ((m{Γv}r ρ)⇨(m{Γv}r τ)).
-Proof.
-  msubst_tac.
-Qed.
-
-Lemma msubst_flip_rty: forall (Γv: env) τ,
-    closed_env Γv ->
-    m{Γv}r (flip_rty τ) = flip_rty (m{Γv}r τ).
-Proof.
-  destruct τ; simpl flip_rty; intros; eauto.
-  - rewrite msubst_overrty by eauto.
-    rewrite msubst_underrty; eauto.
-  - rewrite msubst_overrty by eauto.
-    rewrite msubst_underrty; eauto.
-  - rewrite msubst_arrrty; eauto.
-Qed.
-
-(* Tactic Notation "rewrite_msubst" constr(lem) "in" hyp(H) := *)
-(*   rewrite lem in H; eauto using ctxRst_closed_env. *)
-
-(* Tactic Notation "rewrite_msubst" constr(lem) := *)
-(*   rewrite lem in *; eauto using ctxRst_closed_env. *)
-
-Lemma msubst_mk_top: forall (Γv: env) b,
-    closed_env Γv ->
-    m{Γv}r (mk_top b) = mk_top b.
-Proof.
-  intros.
-  unfold mk_top, mk_q_under_top.
-  rewrite msubst_underrty in *; eauto. f_equal.
-  rewrite msubst_qualifier in *; eauto.
-Qed.
-
-Lemma msubst_mk_eq_constant: forall (Γv: env) c,
-    closed_env Γv ->
-    (m{Γv}r) (mk_eq_constant c) = (mk_eq_constant c).
-Proof.
-  intros.
-  unfold mk_eq_constant, mk_q_bvar_eq_val.
-  repeat rewrite msubst_underrty; eauto. f_equal.
-  repeat rewrite msubst_qualifier; eauto. f_equal.
-  simpl.
-  repeat rewrite msubst_bvar.
-  repeat rewrite msubst_constant. eauto.
-Qed.
-
-Lemma msubst_mk_eq_var: forall (Γv: env) b x v,
-    closed_env Γv ->
-    Γv !! x = Some v ->
-    (m{Γv}r) (mk_eq_var b x) = [:b | b0:v= v].
-Proof.
-  intros.
-  unfold mk_eq_var.
-  repeat rewrite msubst_underrty; eauto.
-  repeat rewrite msubst_qualifier; eauto.
-  simpl.
-  repeat rewrite msubst_bvar; eauto.
-  repeat rewrite msubst_fvar; eauto.
-  rewrite H0.
-  eauto.
-Qed.
-
-Ltac msubst_simp :=
-  match goal with
-  | H: context [ m{ _ }t (tlete _ _) ] |- _ => rewrite msubst_lete in H
-  | |- context [ m{ _ }t (tlete _ _) ] => rewrite msubst_lete
-  | H: context [ m{ _ }t (tleteffop _ _ _) ] |- _ => rewrite msubst_tleteffop in H
-  | |- context [ m{ _ }t (tleteffop _ _ _) ] => rewrite msubst_tleteffop
-  | H: context [ m{ _ }t (tletapp _ _ _) ] |- _ => rewrite msubst_tletapp in H
-  | |- context [ m{ _ }t (tletapp _ _ _) ] => rewrite msubst_tletapp
-  | H: context [ m{ _ }v (vfix _ _) ] |- _ => rewrite msubst_fix in H
-  | |- context [ m{ _ }v (vfix _ _) ] => rewrite msubst_fix
-  | H: context [ m{ _ }t (treturn _) ] |- _ => rewrite msubst_value in H
-  | |- context [ m{ _ }t (treturn _) ] => rewrite msubst_value
-  | H: context [ m{ _ }v (vlam _ _) ] |- _ => rewrite msubst_lam in H
-  | |- context [ m{ _ }v (vlam _ _) ] => rewrite msubst_lam
-  | H: context [ m{ _ }t (tmatchb _ _ _) ] |- _ => rewrite msubst_match in H
-  | |- context [ m{ _ }t (tmatchb _ _ _) ] => rewrite msubst_match
-  | H: context [ m{ _ }v (vbvar _) ] |- _ => rewrite msubst_bvar in H
-  | |- context [ m{ _ }v (vbvar _) ] => rewrite msubst_bvar
-  | H: context [ m{ _ }v (vfvar _) ] |- _ => rewrite msubst_fvar in H
-  | |- context [ m{ _ }v (vfvar _) ] => rewrite msubst_fvar
-  | H: context [ m{ _ }v (vconst _) ] |- _ => rewrite msubst_constant in H
-  | |- context [ m{ _ }v (vconst _) ] => rewrite msubst_constant
-  (* NOTE: don't unfold qualifier definition *)
-  (* | H: context [ m{ _ }q _ ] |- _ => rewrite msubst_qualifier in H *)
-  (* | |- context [ m{ _ }q _ ] => rewrite msubst_qualifier *)
-  | H: context [ m{ _ }q (_ & _) ] |- _ => rewrite msubst_qualifier_and in H
-  | |- context [ m{ _ }q (_ & _) ] => rewrite msubst_qualifier_and
-  | H: context [ m{ _ }r {: _ | _ } ] |- _ => rewrite msubst_overrty in H
-  | |- context [ m{ _ }r {: _ | _ } ] => rewrite msubst_overrty
-  | H: context [ m{ _ }r [: _ | _ ] ] |- _ => rewrite msubst_underrty in H
-  | |- context [ m{ _ }r [: _ | _ ] ] => rewrite msubst_underrty
-  | H: context [ m{ _ }r (_ ⇨ _) ] |- _ => rewrite msubst_arrrty in H
-  | |- context [ m{ _ }r (_ ⇨ _ ) ] => rewrite msubst_arrrty
-  | H: context [ m{ _ }r (mk_top _) ] |- _ => rewrite msubst_mk_top in H
-  | |- context [ m{ _ }r (mk_top _) ] => rewrite msubst_mk_top
-  | H: context [ m{ _ }r (mk_eq_constant _) ] |- _ => rewrite msubst_mk_eq_constant in H
-  | |- context [ m{ _ }r (mk_eq_constant _) ] => rewrite msubst_mk_eq_constant
-  | H: context [ m{ _ }r (flip_rty _) ] |- _ => rewrite msubst_flip_rty in H
-  | |- context [ m{ _ }r (flip_rty _) ] => rewrite msubst_flip_rty
-  | H: context [ m{ _ }r (mk_eq_var _ ?x) ], H': _ !! ?x = Some ?v |- _ => rewrite msubst_mk_eq_var with (v:=v) in H
-  | H': _ !! ?x = Some ?v |- context [ m{ _ }r (mk_eq_var _ ?x) ] => rewrite msubst_mk_eq_var with (v:=v)
-  end; eauto.
-
-
-(* Most lemmas here are generalization of the corresponding lemmas about
-single-substitution. *)
-
-Lemma msubst_open_var_tm: forall (Γv: env) e k (x: atom),
-    closed_env Γv ->
-    map_Forall (fun _ v => lc (treturn v)) Γv ->
-    x ∉ dom Γv ->
-    (m{Γv}t) ({k ~t> x} e) = {k ~t> x} ((m{Γv}t) e).
-Proof.
-    msubst_tac.
-    apply map_Forall_insert in H3; eauto.
-    setoid_rewrite H7; eauto.
-    apply subst_open_var_tm. my_set_solver.
-    qauto. qauto.
-    my_set_solver.
-Qed.
-
-Lemma msubst_open_rty: forall (Γv: env) (ρ: rty) k (v_x: value),
-    closed_env Γv ->
-    map_Forall (fun _ v => lc (treturn v)) Γv ->
-    (m{Γv}r) ({k ~r> v_x} ρ) = {k ~r> (m{Γv}v v_x)} (m{Γv}r ρ).
-Proof.
-  msubst_tac.
-  apply map_Forall_insert in H3; eauto. simp_hyps.
-  fold_forward.
-  by apply subst_open_rty.
-Qed.
-
-Lemma msubst_fresh_qualifier Γv ϕ :
-  dom Γv ## qualifier_fv ϕ -> (m{Γv}q) ϕ = ϕ.
-Proof.
-  msubst_tac.
-  pose subst_fresh_qualifier.
-  setoid_rewrite H1; my_set_solver.
-Qed.
-
-Lemma msubst_fresh_rty Γv ρ :
-  dom Γv ## rty_fv ρ ->
-  (m{Γv}r) ρ = ρ.
-Proof.
-  msubst_tac.
-  pose subst_fresh_rty.
-  setoid_rewrite H1; my_set_solver.
-Qed.
-
-Lemma msubst_fresh_value Γv v :
-  dom Γv ## fv_value v ->
-  (m{Γv}v) v = v.
-Proof.
-  msubst_tac.
-  pose subst_fresh_value.
-  setoid_rewrite H1; my_set_solver.
-Qed.
-
-(* The proof can be reduced to [msubst_open_var_tm] and [msubst_fresh_tm]
-(haven't defined yet; see [msubst_fresh_rty] for example). It's a pain to define
-those for every [msubst_intro_*]. Don't bother yet. *)
-Lemma msubst_intro_tm: forall (Γv: env) e k (v_x: value) (x: atom),
-    closed_env Γv ->
-    closed_value v_x ->
-    map_Forall (fun _ v => lc (treturn v)) Γv ->
-    x ∉ dom Γv ∪ stale e ->
-    {k ~t> v_x} ((m{Γv}t) e) = (m{<[x:=v_x]> Γv}t) ({k ~t> x} e).
-Proof.
-  intros.
-  rewrite_msubst_insert.
-  2 : apply not_elem_of_dom; my_set_solver.
-  revert_all.
-  intros *.
-  msubst_tac.
-  - repeat rewrite map_fold_empty. rewrite open_subst_same_tm; my_set_solver.
-  - apply map_Forall_insert in H4; eauto.
-    rewrite subst_commute_tm by my_set_solver.
-    rewrite <- subst_open_tm_closed by my_set_solver. f_equal.
-    setoid_rewrite H1; eauto. qauto. my_set_solver.
-Qed.
-
-Lemma msubst_intro_value: forall (Γv: env) (v: value) k (v_x: value) (x: atom),
-    closed_env Γv ->
-    closed_value v_x ->
-    map_Forall (fun _ v => lc (treturn v)) Γv ->
-    x ∉ dom Γv ∪ stale v ->
-    {k ~v> v_x} ((m{Γv}v) v) = (m{<[x:=v_x]> Γv}v) ({k ~v> x} v).
-Proof.
-  intros.
-  rewrite_msubst_insert.
-  2 : apply not_elem_of_dom; my_set_solver.
-  revert_all.
-  intros *.
-  msubst_tac.
-  - repeat rewrite map_fold_empty. rewrite open_subst_same_value. auto. my_set_solver.
-  - apply map_Forall_insert in H4; eauto.
-    rewrite subst_commute_value by my_set_solver.
-    rewrite <- subst_open_value_closed by my_set_solver. f_equal.
-    setoid_rewrite H1; eauto. qauto. my_set_solver.
-Qed.
-
-Lemma msubst_intro_rty: forall (Γv: env) e k (v_x: value) (x: atom),
-    closed_env Γv ->
-    closed_value v_x ->
-    map_Forall (fun _ v => lc (treturn v)) Γv ->
-    x ∉ dom Γv ∪ stale e ->
-    {k ~r> v_x} ((m{Γv}r) e) = (m{<[x:=v_x]> Γv}r) ({k ~r> x} e).
-Proof.
-  intros.
-  rewrite_msubst_insert.
-  2 : apply not_elem_of_dom; my_set_solver.
-  revert_all.
-  intros *.
-  msubst_tac.
-  - repeat rewrite map_fold_empty. rewrite open_subst_same_rty. auto. my_set_solver.
-  - apply map_Forall_insert in H4; eauto.
-    rewrite subst_commute_rty by my_set_solver.
-    rewrite <- subst_open_rty_closed by my_set_solver. f_equal.
-    setoid_rewrite H1; eauto. qauto. my_set_solver.
-Qed.
-
-Lemma msubst_intro_qualifier: forall (Γv: env) e k (v_x: value) (x: atom),
-    closed_env Γv ->
-    closed_value v_x ->
-    map_Forall (fun _ v => lc (treturn v)) Γv ->
-    x ∉ dom Γv ∪ stale e ->
-    {k ~q> v_x} ((m{Γv}q) e) = (m{<[x:=v_x]> Γv}q) ({k ~q> x} e).
-Proof.
-  intros.
-  rewrite_msubst_insert.
-  2 : apply not_elem_of_dom; my_set_solver.
-  revert_all.
-  intros *.
-  msubst_tac.
-  - repeat rewrite map_fold_empty. rewrite open_subst_same_qualifier. auto. my_set_solver.
-  - apply map_Forall_insert in H4; eauto.
-    rewrite subst_commute_qualifier by my_set_solver.
-    rewrite <- subst_open_qualifier_closed by my_set_solver. f_equal.
-    setoid_rewrite H1; eauto. qauto. my_set_solver.
-Qed.
-
-Lemma msubst_rty_fv_subseteq Γv ρ:
-  closed_env Γv ->
-  rty_fv (m{Γv}r ρ) ⊆ rty_fv ρ.
-Proof.
-  msubst_tac.
-  rewrite fv_of_subst_rty_closed; my_set_solver.
-Qed.
-
-Lemma msubst_qualifier_fv_subseteq Γv ϕ:
-  closed_env Γv ->
-  qualifier_fv (m{Γv}q ϕ) ⊆ qualifier_fv ϕ.
-Proof.
-  msubst_tac.
-  rewrite fv_of_subst_qualifier_closed by eauto. my_set_solver.
-Qed.
-
-Lemma msubst_tm_fv_subseteq Γv t:
-  closed_env Γv ->
-  fv_tm (m{Γv}t t) ⊆ fv_tm t.
-Proof.
-  msubst_tac.
-  rewrite fv_of_subst_tm by eauto. my_set_solver.
-Qed.
-
-Lemma msubst_value_fv_subseteq Γv (v : value):
-  closed_env Γv ->
-  fv_value (m{Γv}v v) ⊆ fv_tm v.
-Proof.
-  msubst_tac.
-  rewrite fv_of_subst_value by eauto. my_set_solver.
-Qed.
-
-Lemma msubst_insert_fresh_rty Γv x v_x ρ:
-  closed_env Γv ->
-  closed_value v_x ->
-  x ∉ dom Γv ∪ rty_fv ρ ->
-  (m{<[x:=v_x]> Γv}r) ρ = (m{Γv}r) ρ.
-Proof.
-  intros.
-  rewrite_msubst_insert. 2: apply not_elem_of_dom; my_set_solver.
-  apply subst_fresh_rty.
-  eapply not_elem_of_weaken; eauto.
-  rewrite msubst_rty_fv_subseteq by eauto. my_set_solver.
-Qed.
-
-Lemma msubst_insert_fresh_qualifier Γv x v_x ϕ:
-  closed_env Γv ->
-  closed_value v_x ->
-  x ∉ dom Γv ∪ qualifier_fv ϕ ->
-  (m{<[x:=v_x]> Γv}q) ϕ = (m{Γv}q) ϕ.
-Proof.
-  intros.
-  rewrite_msubst_insert. 2: apply not_elem_of_dom; my_set_solver.
-  apply subst_fresh_qualifier.
-  eapply not_elem_of_weaken; eauto.
-  rewrite msubst_qualifier_fv_subseteq by eauto. my_set_solver.
-Qed.
-
-Lemma msubst_insert_fresh_tm Γv x v_x t:
-  closed_env Γv ->
-  closed_value v_x ->
-  x ∉ dom Γv ∪ fv_tm t ->
-  (m{<[x:=v_x]> Γv}t) t = (m{Γv}t) t.
-Proof.
-  intros.
-  rewrite_msubst_insert. 2: apply not_elem_of_dom; my_set_solver.
-  apply subst_fresh_tm.
-  eapply not_elem_of_weaken; eauto.
-  rewrite msubst_tm_fv_subseteq by eauto. my_set_solver.
-Qed.
-
-Lemma msubst_insert_fresh_value Γv x v_x (v : value):
-  closed_env Γv ->
-  closed_value v_x ->
-  x ∉ dom Γv ∪ fv_tm v ->
-  (m{<[x:=v_x]> Γv}v) v = (m{Γv}v) v.
-Proof.
-  intros.
-  rewrite_msubst_insert. 2: apply not_elem_of_dom; my_set_solver.
-  apply subst_fresh_value.
-  eapply not_elem_of_weaken; eauto.
-  rewrite msubst_value_fv_subseteq by eauto. my_set_solver.
-Qed.
-
-Lemma lc_msubst_rty Γv (ρ: rty):
-  lc_rty (m{Γv}r ρ) ->
-  map_Forall (fun _ v => lc (treturn v)) Γv ->
-  lc_rty ρ.
-Proof.
-  msubst_tac.
-  apply map_Forall_insert in H3; eauto. simp_hyps.
-  eauto using lc_subst_rty.
-Qed.
-
-Lemma msubst_lc_rty Γv (ρ: rty):
-  lc_rty ρ ->
-  map_Forall (fun _ v => lc (treturn v)) Γv ->
-  lc_rty (m{Γv}r ρ).
-Proof.
-  msubst_tac.
-  apply map_Forall_insert in H3; eauto. simp_hyps.
-  eauto using subst_lc_rty.
-Qed.
-
-Lemma rtyR_msubst_insert_eq Γv ρ v x u :
-  closed_env Γv ->
-  closed_value u ->
-  Γv !! x = None ->
-  (⟦(m{ Γv }r) ρ⟧) v ->
-  (⟦(m{ <[x:=u]> Γv }r) ρ⟧) v.
-Proof.
-  intros. rewrite_msubst_insert.
-  rewrite subst_fresh_rty. auto.
-  select (⟦_⟧ _) (fun H => apply rtyR_typed_closed in H).
-  simp_hyps. select (closed_rty _ _) (fun H => sinvert H). my_set_solver.
-Qed.
-
-Lemma fv_of_msubst_rty_closed Γv ρ:
-  closed_env Γv ->
-  rty_fv (m{Γv}r ρ) = rty_fv ρ ∖ dom Γv.
-Proof.
-  revert Γv.
-  msubst_tac.
- my_set_solver.
-  rewrite fv_of_subst_rty_closed by eauto.
-  rewrite dom_insert_L. my_set_solver.
-Qed.
-
-(* Lemma msubst_preserves_closed_rty Γ epr Γv Γ' ρ : *)
-(*   ctxRst Γ epr -> eprR epr Γv ->> *)
-(*   closed_rty (ctxdom (Γ ++ Γ')) ρ -> *)
-(*   closed_rty (ctxdom (Γ')) (m{Γv}r ρ). *)
-(* Proof. *)
-(*   intros HΓv HP H. *)
-(*   sinvert H. *)
-(*   econstructor. eauto using msubst_lc_rty, ctxRst_lc. *)
-(*   rewrite fv_of_msubst_rty_closed by eauto using ctxRst_closed_env. *)
-(*   rewrite ctxdom_app_union in *. *)
-(*   rewrite ctxRst_dom in * by eauto. *)
-(*   my_set_solver. *)
-(* Qed. *)
-
-(* Lemma msubst_preserves_closed_rty_empty Γ epr Γv ρ : *)
-(*   ctxRst Γ epr -> eprR epr Γv ->> *)
-(*   closed_rty (ctxdom Γ) ρ -> *)
-(*   closed_rty ∅ (m{Γv}r ρ). *)
-(* Proof. *)
-(*   intros. eapply msubst_preserves_closed_rty with (Γ':=[]); eauto. *)
-(*   by simplify_list_eq. *)
-(* Qed. *)
-
-Lemma msubst_preserves_rty_measure ρ Γv:
-  rty_measure ρ = rty_measure (m{Γv}r ρ).
+Lemma msubst_preserves_rty_measure ρ: forall σ: env,
+  rty_measure ρ = rty_measure (m{σ} ρ).
 Proof.
   msubst_tac. qauto using subst_preserves_rty_measure.
 Qed.
 
-Lemma msubst_preserves_basic_typing_tm Γ epr Γv :
-  ctxRst Γ epr -> eprR epr Γv ->
-  forall Γ' e T,
-    (⌊Γ⌋* ∪ Γ') ⊢t e ⋮t T ->
-    Γ' ⊢t m{Γv}t e ⋮t T.
+Lemma rtyR_msubst_insert_eq (σ: env) (ρ: rty) (v: tm) (x: atom) (u: value):
+  closed_env σ ->
+  stale u = ∅ ->
+  σ !! x = None ->
+  (⟦(m{ σ }) ρ⟧) v ->
+  (⟦(m{ <[x:=u]> σ }) ρ⟧) v.
 Proof.
-  intros H HP.
-  induction 1; intros; eauto.
-  - repeat msubst_simp.
-(*   apply_eq H. cbn. apply map_empty_union. *)
-(*   rewrite ctx_erase_app in H2. *)
-(*   rewrite <- map_union_assoc in H2. *)
-(*   apply IHctxRst in H2. *)
-(*   rewrite msubst_insert; *)
-(*     eauto using subst_commute_tm, ctxRst_closed_env, *)
-(*                 rtyR_closed_value, ctxRst_ok_insert. *)
-(*   eapply basic_typing_subst_tm; cycle 1. *)
-(*   eapply_eq H2. *)
-(*   cbn. rewrite map_union_empty. rewrite insert_empty. *)
-(*   rewrite <- insert_union_singleton_l. reflexivity. *)
-(*   eapply basic_typing_weaken_value. apply map_empty_subseteq. *)
-(*   apply rtyR_typed_closed in H1. simp_hyps. *)
-(*   sinvert H1. apply_eq H6. eauto using rty_erase_msubst_eq. *)
-(* Qed. *)
-Admitted.
-
-Lemma msubst_preserves_basic_typing_value Γ epr Γv :
-  ctxRst Γ epr -> eprR epr Γv ->
-  forall Γ' v T,
-    (⌊Γ⌋* ∪ Γ') ⊢t v ⋮v T ->
-    Γ' ⊢t m{Γv}v v ⋮v T.
-Proof.
-  induction 1; intros; eauto.
-Admitted.
-(*   apply_eq H. cbn. apply map_empty_union. *)
-(*   rewrite ctx_erase_app in H2. *)
-(*   rewrite <- map_union_assoc in H2. *)
-(*   apply IHctxRst in H2. *)
-(*   rewrite msubst_insert; *)
-(*     eauto using subst_commute_value, ctxRst_closed_env, *)
-(*     rtyR_closed_value, ctxRst_ok_insert. *)
-(*   eapply basic_typing_subst_value; cycle 1. *)
-(*   eapply_eq H2. *)
-(*   cbn. rewrite map_union_empty. rewrite insert_empty. *)
-(*   rewrite <- insert_union_singleton_l. reflexivity. *)
-(*   eapply basic_typing_weaken_value. apply map_empty_subseteq. *)
-(*   apply rtyR_typed_closed in H1. simp_hyps. *)
-(*   sinvert H1. apply_eq H6. eauto using rty_erase_msubst_eq. *)
-(* Qed. *)
-
-Lemma msubst_preserves_basic_typing_tm_empty Γ epr Γv :
-  ctxRst Γ epr -> eprR epr Γv ->
-  forall e T,
-    ( ⌊Γ⌋* ) ⊢t e ⋮t T ->
-    ∅ ⊢t m{Γv}t e ⋮t T.
-Proof.
-  intros. eapply msubst_preserves_basic_typing_tm; eauto.
-  rewrite map_union_empty. eauto.
-Qed.
-
-Lemma msubst_preserves_basic_typing_value_empty Γ epr Γv :
-  ctxRst Γ epr -> eprR epr Γv ->
-  forall v T,
-    ( ⌊Γ⌋* ) ⊢t v ⋮v T ->
-    ∅ ⊢t m{Γv}v v ⋮v T.
-Proof.
-  intros. eapply msubst_preserves_basic_typing_value; eauto.
-  rewrite map_union_empty. eauto.
-Qed.
-
-Lemma fv_of_msubst_value_closed Γv ρ:
-  closed_env Γv ->
-  fv_value (m{Γv}v ρ) = fv_value ρ ∖ dom Γv.
-Proof.
-  revert Γv.
-  msubst_tac.
+  intros. rewrite_msubst_insert.
+  rewrite subst_fresh. auto.
+  select (⟦_⟧ _) (fun H => apply rtyR_typed_closed in H).
+  simp_hyps.
   my_set_solver.
-  rewrite fv_of_subst_value_closed by eauto.
-  rewrite dom_insert_L. my_set_solver.
 Qed.
 
-Lemma fv_of_msubst_tm_closed Γv ρ:
-  closed_env Γv ->
-  fv_tm (m{Γv}t ρ) = fv_tm ρ ∖ dom Γv.
+Lemma ctx_erase_not_fv {A: Type} Γ (x y: atom) (r: A): x # ((y, r) :: Γ) -> x ≠ y /\ x ∉ stale Γ.
 Proof.
-  revert Γv.
-  msubst_tac.
-  my_set_solver.
-  rewrite fv_of_subst_tm_closed by eauto.
-  rewrite dom_insert_L. my_set_solver.
+  intros. ln_simpl. my_set_solver.
+Qed.
+
+Lemma ctx_erase_empty: ⌊[]⌋* = ∅.
+Proof.
+  unfold erase_ctx. simplify_map_eq. reflexivity.
+Qed.
+
+Ltac my_map_simpl :=
+  match goal with
+  | [H: context [ ∅ ∪ _ ] |- _ ] => rewrite map_empty_union in H
+  | [|- context [ ∅ ∪ _ ] ] => rewrite map_empty_union
+  | [H: context [ _ ∪ ∅ ] |- _ ] => rewrite map_union_empty in H
+  | [|- context [ _ ∪ ∅ ] ] => rewrite map_union_empty
+  end.
+
+Lemma flip_rty_erase_msubst_eq τ: ⌊flip_rty τ⌋ = ⌊τ⌋.
+Proof.
+  induction τ; simpl; eauto.
+Qed.
+
+Ltac simplify_erase_aux1 :=
+  match goal with
+  | [H: context [ ⌊ flip_rty _ ⌋ ] |- _ ] => setoid_rewrite ->flip_rty_erase_msubst_eq in H
+  | [H: _ |- context [ ⌊ flip_rty _ ⌋ ]] => setoid_rewrite ->  flip_rty_erase_msubst_eq
+  | [H: context [ ⌊ m{_} _ ⌋ ] |- _ ] => setoid_rewrite <- rty_erase_msubst_eq in H 
+    | [H: _ |- context [ ⌊ m{_} _ ⌋ ]] => setoid_rewrite <- rty_erase_msubst_eq
+  | [H: context [ ⌊[]⌋* ] |- _ ] => rewrite ctx_erase_empty in H
+  | [|- ⌊[]⌋* = _ ] => rewrite ctx_erase_empty
+  | [|- _ !! _ = None] => apply not_elem_of_dom; fold_syntax_class
+  | [H: context [ stale (⌊ _ ⌋*) ] |- _ ] => rewrite ctx_erase_dom in H
+  | [|- context [ stale (⌊ _ ⌋*) ] ] => rewrite ctx_erase_dom
+  | [H: context [ _ # (⌊ _ ⌋*) ] |- _ ] => 
+    rewrite ctx_erase_dom in H by eauto
+  | [|- context [ _ # (⌊ _ ⌋*) ] ] => rewrite ctx_erase_dom by eauto
+  | [H: context [ ⌊_ :: ?Γ⌋* ] |- _ ] => rewrite ctx_erase_cons in H by eauto
+  | [|- context [ ⌊_ :: ?Γ⌋* ] ] => rewrite ctx_erase_cons by eauto
+  | [H: context [ ⌊?Γ ++ [_]⌋* ] |- _ ] => rewrite ctx_erase_app_r in H by eauto
+  | [|- context [ ⌊?Γ ++ [_]⌋* ] ] => rewrite ctx_erase_app_r by eauto
+  | [H: context [ ⌊?Γ ++ ?Γ'⌋* ] |- _ ] => rewrite ctx_erase_app in H by eauto
+  | [|- context [ ⌊?Γ ++ ?Γ'⌋* ] ] => rewrite ctx_erase_app by eauto
+  | _ => my_map_simpl
+  end.
+
+Ltac simplify_erase1 :=
+  mydestr;
+  repeat (simplify_erase_aux1; eauto).
+
+Lemma ctx_erase_lookup_none:
+forall (Γ : listctx rty) (x : atom), x # Γ -> ⌊Γ⌋* !! x = None.
+Proof.
+  induction Γ; intros; simpl; try easy.
+  simplify_erase1.
+Qed.
+
+(* Ltac simplify_erase_aux2 :=
+  match goal with
+  (* | [H: ?x # ((_, _) :: _) |- ?x # _] => apply ctx_erase_not_fv in H; mydestr *)
+  end. *)
+
+(* Ltac simplify_erase :=
+  listctx_set_simpl;
+  repeat simplify_erase_aux. *)
+
+Ltac apply_rev_ind :=
+    intros_until (listctx rty);
+    lazymatch goal with
+    | |- forall Γ : listctx rty, ?body =>
+        let P := constr:(fun Γ : listctx rty => body) in
+        apply (List.rev_ind P); intros
+    end.
+
+Lemma ctxEnv_destruct_tail Γ (σ: env) x r:
+  ctxEnv (Γ ++ [(x, r)]) σ ->
+  exists (v: value) (σ': env), σ = <[x:=v]> σ' /\ ctxEnv Γ σ' /\ (⟦(m{σ'}) (flip_rty r)⟧) (treturn v) /\ ok_ctx (Γ ++ [(x, r)]).
+Proof.
+  intros. sinvert H.
+  - listctx_set_solver.
+  - listctx_set_simpl. exists v, σ0. intuition.
+Qed.
+
+Ltac set_simp_aux :=
+  match goal with
+     | [H: ⟦ _ ⟧ _ |- stale _ = _ ] => apply rtyR_typed_closed in H; simp_hyp H
+     | [H: ⟦ _ ⟧ _ |- _ !! _ = _ ] => apply rtyR_typed_closed in H; simp_hyp H
+     | [H: ⟦ _ ⟧ _ |- _ # _ ] => apply rtyR_typed_closed in H; simp_hyp H
+     | [H: _ ⊢r _ ⋮ _ |- stale _ = _ ] => apply refinement_typing_regular in H
+     | [H: _ ⊢ _ ⋮ _ |- stale _ = _ ] => apply fv_subset_gamma in H
+     end.
+
+Ltac set_simp := repeat set_simp_aux.
+
+
+Ltac rtyR_regular_simp_aux :=
+  match goal with
+     | [H: ctxEnv _ _ |- lc _ ] => apply ctxEnv_regular in H; simp_hyp H
+     | [H: ctxEnv _ _ |- closed_env _ ] => apply ctxEnv_regular in H; simp_hyp H
+     | [H: ctxEnv _ _ |- ok_ctx _ ] => apply ctxEnv_regular in H; simp_hyp H; eauto
+     | [H: ctxEnv _ _ |- _ ∉ _ ] => apply ctxEnv_regular in H; simp_hyp H; eauto
+     | [H: ctxEnv _ _ |- _ # _ ] => apply ctxEnv_regular in H; simp_hyp H; eauto
+     | [H: ctxEnv _ _ |- _ ⊆ _ ] => apply ctxEnv_regular in H; eauto; simp_hyp H
+     | [H: ctxEnv _ _ |- stale _ = _ ] => apply ctxEnv_regular in H; eauto; simp_hyp H
+     | [H: ctxEnv _ _ |- _ !! _ = _ ] => apply ctxEnv_regular in H; eauto; simp_hyp H
+     | [H: ctxEnv _ ?Γv |- map_Forall _ ?Γv] => apply ctxEnv_regular in H; eauto
+     | [H: ⟦ _ ⟧ _  |- lc _ ] => apply rtyR_regular in H; simp_hyp H
+     | [H: ⟦ _ ⟧ _  |- _ ⊆ _ ] => apply rtyR_regular in H; eauto; simp_hyp H
+     | [H: ⟦ _ ⟧ _  |- stale _ = _ ] => apply rtyR_regular in H; eauto; simp_hyp H
+     | [H: ⟦ _ ⟧ _  |- _ ⊢ _ ⋮ _ ] => apply rtyR_typed_closed in H; simp_hyp H
+     end.
+
+Ltac rtyR_regular_simp :=
+  repeat rtyR_regular_simp_aux.
+
+Class MsubstPreservesBasicTyping A `{Stale A} `{Subst value A} `{Typing tyctx A ty} := msubst_preserves_basic_typing :
+  forall Γ (σ: env),
+    ctxEnv Γ σ ->
+    forall Γ' (e: A) T,
+      (⌊Γ⌋* ∪ Γ') ⊢ e ⋮ T ->
+      Γ' ⊢ m{σ} e ⋮ T.
+
+Lemma MsubstPreservesBasicTyping_all
+(A : Type)
+(staleA : Stale A)
+(substA : Subst value A)
+(typingA : @Typing tyctx A ty)
+(msubst_insertA : @MsubstInsert A substA)
+(basic_typing_substA : @BasicTypingSubst A typingA substA)
+: @MsubstPreservesBasicTyping A staleA substA typingA.
+Proof.
+  unfold MsubstPreservesBasicTyping.
+  induction 1; intros; eauto.
+  - simplify_erase1.
+  - apply ok_ctx_destruct_tail in H0. mydestr.
+    simplify_erase1.
+  rewrite_msubst_insert.
+  apply basic_typing_substA with (U := ⌊τ⌋); eauto.
+  apply rtyR_regular in H1. mydestr.
+  + rtyR_regular_simp. simplify_erase1. basic_typing_solver.
+  + 
+  apply IHctxEnv; eauto.
+  rewrite insert_union_singleton_r in H2.
+  setoid_rewrite insert_union_singleton_l.
+  rewrite map_union_assoc. 
+  eauto.
+  simplify_erase1.
+  + rtyR_regular_simp; eauto.
+  + rtyR_regular_simp. lc_set_solver.
+  + rtyR_regular_simp. simplify_erase1. 
+    autounfold with class_simpl in *. hauto. 
+Qed.
+
+#[global] Instance MsubstPreservesBasicTyping_tm: MsubstPreservesBasicTyping tm.
+Proof.
+  eapply MsubstPreservesBasicTyping_all; typeclasses eauto.
+Qed.
+
+#[global] Instance MsubstPreservesBasicTyping_value: MsubstPreservesBasicTyping value.
+Proof.
+  eapply MsubstPreservesBasicTyping_all; typeclasses eauto.
+Qed.
+
+Class MsubstPreservesBasicTypingEmpty A `{Stale A} `{Subst value A} `{Typing tyctx A ty} := msubst_preserves_basic_typing_empty :
+  forall Γ (σ: env),
+    ctxEnv Γ σ ->
+    forall e T,
+    ( ⌊Γ⌋* ) ⊢ e ⋮ T ->
+    ∅ ⊢ m{σ} e ⋮ T.
+
+Lemma MsubstPreservesBasicTypingEmpty_all
+(A : Type)
+(staleA : Stale A)
+(substA : Subst value A)
+(typingA : @Typing tyctx A ty)
+(msubst_preserves_basic_typingA : @MsubstPreservesBasicTyping A staleA substA typingA)
+: @MsubstPreservesBasicTypingEmpty A staleA substA typingA.
+Proof.
+  unfold MsubstPreservesBasicTypingEmpty.
+  intros. eapply msubst_preserves_basic_typingA; eauto.
+  my_map_simpl; eauto.
+Qed.
+
+#[global] Instance MsubstPreservesBasicTypingEmpty_tm: MsubstPreservesBasicTypingEmpty tm.
+Proof.
+  eapply MsubstPreservesBasicTypingEmpty_all; typeclasses eauto.
+Qed.
+
+#[global] Instance MsubstPreservesBasicTypingEmpty_value: MsubstPreservesBasicTypingEmpty value.
+Proof.
+  eapply MsubstPreservesBasicTypingEmpty_all; typeclasses eauto.
 Qed.
 
 From Stdlib Require Import Logic.ClassicalFacts.
 From Stdlib Require Import Classical.
 From Stdlib Require Import Arith.Compare_dec.
 
-Lemma msubst_fvar_inv (Γv : env) v (x : atom) :
-  closed_env Γv ->
-  m{Γv}v v = x ->
-  v = x /\ x ∉ dom Γv.
+Lemma msubst_fvar_inv v (x : atom): forall (σ : env),
+  closed_env σ ->
+  m{σ} v = (treturn (vfvar x)) ->
+  v = (treturn (vfvar x)) /\ x ∉ dom σ.
 Proof.
   msubst_tac; fold_msubst. set_solver.
   rewrite <- H0 in H3.
   destruct v; repeat msubst_simp; inversion H3; subst.
+  destruct v; repeat msubst_simp; inversion H3; subst.
   - destruct (<[i:=x0]> m !! atom) eqn: Hx.
     + exfalso. unfold closed_env in H2.
-      eapply map_Forall_lookup_1 in H2; eauto. unfold closed_value in H2. my_set_solver.
+      eapply map_Forall_lookup_1 in H2; eauto.
+      ln_simpl.
     + split; auto. inversion H3. subst. apply not_elem_of_dom in Hx. eauto.
 Qed.
 
-Lemma msubst_destruct_rev_tm: forall (Γv: env) (x: atom) (v_x: value) (e: tm),
-    closed_env Γv -> closed_value v_x -> x ∉ dom Γv ->
-    (m{<[x:=v_x]> Γv}t) e = m{Γv}t ({ x:=v_x }t e).
+Lemma msubst_destruct_rev_tm: forall (σ: env) (x: atom) (v_x: value) (e: tm),
+    closed_env σ -> stale v_x = ∅ -> x ∉ dom σ ->
+    (m{<[x:=v_x]> σ}) e = m{σ} ({ x:=v_x } e).
 Proof.
   intros.
   rewrite_msubst_insert.
@@ -764,7 +334,7 @@ Proof.
 Qed.
 
 Lemma is_coverage_rty_msubst_aux n : forall τ, rty_measure τ <= n ->
-                                         forall Γv, closed_env Γv -> is_coverage_rty (m{ Γv }r τ) <-> is_coverage_rty τ.
+                                         forall σ, closed_env σ -> is_coverage_rty (m{ σ } τ) <-> is_coverage_rty τ.
 Proof.
   induction n; split; intros Hm; simpl; intros; repeat msubst_simp; simp_hyps; eauto.
   - pose (rty_measure_gt_0 τ). lia.
@@ -787,10 +357,10 @@ Proof.
       * eapply H1; eauto. simpl in *. lia. sinvert Hm; eauto.
 Qed.
 
-Lemma is_coverage_rty_msubst: forall τ Γv, closed_env Γv -> is_coverage_rty (m{ Γv }r τ) <-> is_coverage_rty τ.
+Lemma is_coverage_rty_msubst: forall τ σ, closed_env σ -> is_coverage_rty (m{ σ } τ) <-> is_coverage_rty τ.
 Proof. eauto using is_coverage_rty_msubst_aux. Qed.
 
-Lemma fine_rty_msubst: forall τ Γv, closed_env Γv -> fine_rty (m{ Γv }r τ) <-> fine_rty τ.
+Lemma fine_rty_msubst: forall τ σ, closed_env σ -> fine_rty (m{ σ } τ) <-> fine_rty τ.
 Proof.
   split; destruct τ; intros; repeat msubst_simp; simp_hyps; eauto; simpl in *.
   - erewrite <- is_coverage_rty_msubst; eauto. repeat msubst_simp; simp_hyps; eauto.
@@ -799,25 +369,63 @@ Qed.
 
 Ltac fine_rty_simp_aux :=
   match goal with
-  | [H: context [ fine_rty (m{_}r ?τ) ] |- _ ] => setoid_rewrite fine_rty_msubst in H
-  | [H: _ |- context [ fine_rty (m{_}r ?τ) ] ] => setoid_rewrite fine_rty_msubst
-  | [H: context [ is_coverage_rty (m{_}r ?τ) ] |- _ ] => setoid_rewrite is_coverage_rty_msubst in H
-  | [H: _ |- context [ is_coverage_rty (m{_}r ?τ) ] ] => setoid_rewrite is_coverage_rty_msubst
-  (* | [H: context [ is_tm_rty (m{_}r ?τ) ] |- _ ] => setoid_rewrite is_tm_rty_msubst in H *)
-  (* | [H: _ |- context [ is_tm_rty (m{_}r ?τ) ] ] => setoid_rewrite is_tm_rty_msubst *)
-  (* | [H: context [ pure_rty (m{_}r ?τ) ] |- _ ] => setoid_rewrite pure_rty_msubst in H *)
-  (* | [H: _ |- context [ pure_rty (m{_}r ?τ) ] ] => setoid_rewrite pure_rty_msubst *)
+  | [H: context [ fine_rty (m{_} ?τ) ] |- _ ] => setoid_rewrite fine_rty_msubst in H
+  | [H: _ |- context [ fine_rty (m{_} ?τ) ] ] => setoid_rewrite fine_rty_msubst
+  | [H: context [ is_coverage_rty (m{_} ?τ) ] |- _ ] => setoid_rewrite is_coverage_rty_msubst in H
+  | [H: _ |- context [ is_coverage_rty (m{_} ?τ) ] ] => setoid_rewrite is_coverage_rty_msubst
+  (* | [H: context [ is_tm_rty (m{_} ?τ) ] |- _ ] => setoid_rewrite is_tm_rty_msubst in H *)
+  (* | [H: _ |- context [ is_tm_rty (m{_} ?τ) ] ] => setoid_rewrite is_tm_rty_msubst *)
+  (* | [H: context [ pure_rty (m{_} ?τ) ] |- _ ] => setoid_rewrite pure_rty_msubst in H *)
+  (* | [H: _ |- context [ pure_rty (m{_} ?τ) ] ] => setoid_rewrite pure_rty_msubst *)
   end.
 
 Ltac msubst_simp_tac :=
   repeat (match goal with
-          | [H: context [ fine_rty (m{_}r ?τ) ] |- _ ] => setoid_rewrite fine_rty_msubst in H
-          | [H: _ |- context [ fine_rty (m{_}r ?τ) ] ] => setoid_rewrite fine_rty_msubst
-          | [H: context [ is_coverage_rty (m{_}r ?τ) ] |- _ ] => setoid_rewrite is_coverage_rty_msubst in H
-          | [H: _ |- context [ is_coverage_rty (m{_}r ?τ) ] ] => setoid_rewrite is_coverage_rty_msubst
-          (* | [H: context [ is_tm_rty (m{_}r ?τ) ] |- _ ] => setoid_rewrite is_tm_rty_msubst in H *)
-          (* | [H: _ |- context [ is_tm_rty (m{_}r ?τ) ] ] => setoid_rewrite is_tm_rty_msubst *)
-          (* | [H: context [ pure_rty (m{_}r ?τ) ] |- _ ] => setoid_rewrite pure_rty_msubst in H *)
-          (* | [H: _ |- context [ pure_rty (m{_}r ?τ) ] ] => setoid_rewrite pure_rty_msubst *)
+          | [H: context [ fine_rty (m{_} ?τ) ] |- _ ] => setoid_rewrite fine_rty_msubst in H
+          | [H: _ |- context [ fine_rty (m{_} ?τ) ] ] => setoid_rewrite fine_rty_msubst
+          | [H: context [ is_coverage_rty (m{_} ?τ) ] |- _ ] => setoid_rewrite is_coverage_rty_msubst in H
+          | [H: _ |- context [ is_coverage_rty (m{_} ?τ) ] ] => setoid_rewrite is_coverage_rty_msubst
+          (* | [H: context [ is_tm_rty (m{_} ?τ) ] |- _ ] => setoid_rewrite is_tm_rty_msubst in H *)
+          (* | [H: _ |- context [ is_tm_rty (m{_} ?τ) ] ] => setoid_rewrite is_tm_rty_msubst *)
+          (* | [H: context [ pure_rty (m{_} ?τ) ] |- _ ] => setoid_rewrite pure_rty_msubst in H *)
+          (* | [H: _ |- context [ pure_rty (m{_} ?τ) ] ] => setoid_rewrite pure_rty_msubst *)
           | _ => msubst_simp
           end).
+
+(* Ltac fine_solver_aux :=
+  solve [repeat (match goal with
+                 | [ H: _ ⊢WF _ |- fine_rty _ ] =>
+                     apply closed_rty_fine in H; eauto; simpl in H;intuition; eauto
+                 end)].
+
+Ltac fine_solver :=
+  match goal with
+  | [H: _ |- fine_rty _ ] => fine_solver_aux
+  end. *)
+
+(* Ltac basic_typing_simp :=
+  repeat match goal with
+    | [H: ?Γ ⊢ _ ⋮v _ |- ⌊?Γ⌋* ⊢ _ ⋮ _ ] => apply value_typing_regular_basic_typing in H; simpl in H
+    | [H: ?Γ ⊢ _ ⋮v _ |- ⌊?Γ⌋* ⊢ _ ⋮v _ ] => apply value_typing_regular_basic_typing in H; simpl in H
+    | [H: ?Γ ⊢ _ ⋮ _ |- ⌊?Γ⌋* ⊢ _ ⋮ _ ] => apply tm_typing_regular_basic_typing in H; simpl in H
+    | [H: ?Γ ⊢ _ ⋮ _ |- ⌊?Γ⌋* ⊢ _ ⋮v _ ] => apply tm_typing_regular_basic_typing in H; simpl in H
+    | [H: (_ ⊢ _ ⋮ _) |- (_ ⊢  _ ⋮ _) ] => apply tm_typing_regular_basic_typing in H
+    end. *)
+
+(* Ltac simp_tac :=
+  closed_simp; basic_typing_simp; msubst_erase_simp; basic_typing_regular_simp. *)
+
+(* Ltac closed_solver :=
+  match goal with
+  | [H: _ |- closed_rty _ ] => simp_tac
+  | [H: _ |- closed_env _ ] => simp_tac
+  end. *)
+
+(* Ltac lc_solver :=
+  match goal with
+  | [H: _ |- lc _] => simp_tac; lc_solver_plus
+  end. *)
+
+(* Ltac misc_solver :=
+  repeat msubst_simp;
+  try fine_solver; try ok_solver; try closed_solver; try lc_solver. *)
