Typing.v
@@ -1,22 +1,12 @@
-rom stdpp Require Import mapset.
-From CT Require Import CoreLangProp.
+From stdpp Require Import mapset.
+From stdpp Require Import natmap.
+From Stdlib.Program Require Import Wf.
+From CT Require Import Syntax Lc.
 From CT Require Import OperationalSemantics.
 From CT Require Import BasicTypingProp.
-From CT Require Import RefinementTypeProp.
-From CT Require Import DenotationProp.
-From CT Require Import InstantiationProp.
+From CT Require Import Denotation.
 
-Import Atom.
-Import CoreLang.
-Import Tactics.
-Import NamelessTactics.
-Import ListCtx.
-Import OperationalSemantics.
-Import BasicTyping.
-Import Qualifier.
-Import RefinementType.
-Import Denotation.
-Import Instantiation.
+Import BaseDef Lang MyTactics Primitives OperationalSemantics BasicTyping Qualifier RefinementType Instantiation ListCtx List LangLc Lc QualifierLc Denotation.
 
 
 (** This file formalizes the type system of λᴱ and the main metatheoretic
@@ -24,52 +14,45 @@ Import Instantiation.
 
 (** Well-formedness (Fig. 5) *)
 
-(* Definition wf_rty (Γ: listctx rty) (τ: rty): Prop := closed_rty (ctxdom Γ) τ. *)
-(* | WfOver: forall Γ b ϕ, *)
-(*     closed_rty (ctxdom Γ) {: b | ϕ } -> wf_rty Γ {: b | ϕ } *)
-(* | WfUnder: forall Γ b ϕ a, *)
-(*     closed_rty (ctxdom Γ) [: b | ϕ ]!<[ a ]> -> *)
-(*     wf_td *)
-(*     wf_rty Γ [: b | ϕ ]!<[ a ]> *)
-(* | WfArr: forall Γ ρ τ (L: aset), *)
-(*     wf_rty Γ ρ -> *)
-(*     (forall x, x ∉ L -> wf_rty (Γ ++ [(x, ρ)]) (τ ^h^ x)) -> *)
-(*     wf_rty Γ (ρ ⇨ τ) *)
-(* | WfGhost: forall Γ b ρ (L: aset), *)
-(*     (forall x, x ∉ L -> wf_rty (Γ ++ [(x, mk_top b)]) (ρ ^p^ x)) -> *)
-(*     wf_rty Γ (b ⇢ ρ) *)
 
-Notation " Γ '⊢WF' τ " := (closed_rty (ctxdom Γ) τ /\ is_coverage_rty τ) (at level 20, τ constr, Γ constr).
-
-Reserved Notation "Γ '⊢' e '⋮' τ"  (at level 20).
+Notation " Γ '⊢WF' τ " := (lc τ /\ stale τ ⊆ stale Γ /\ is_coverage_rty τ) (at level 20, τ constr, Γ constr).
 
 (** Semantic subtyping *)
 (* Instead of the syntactic subtyping relation presented in the paper, we use
 semantic subtyping in the mechanization. *)
-Definition subtyping (Γ: listctx rty) (ρ1 ρ2: rty) : Prop :=
+(* Definition subtyping (Γ: listctx rty) (ρ1 ρ2: rty) : Prop :=
   (* Assume [ρ1] and [ρ2] are valid [rty]s. *)
   ⌊ ρ1 ⌋ = ⌊ ρ2 ⌋ /\ (is_coverage_rty ρ1 <-> is_coverage_rty ρ2) /\
-    forall epr, ctxRst Γ epr -> exists Γv, eprR epr Γv -> forall e, ⟦m{ Γv }r ρ1⟧ e → ⟦m{ Γv }r ρ2⟧ e.
+    forall (σ1: env), ⟦ Γ ⟧ σ1 ->
+    exists (σ2: env), ⟦ Γ ⟧ σ2 /\ σ1 ={ ctxOverBindings Γ } σ2 /\
+      (forall (e: tm), ⟦m{ σ1 } ρ1⟧ e -> ⟦m{ σ2 } ρ2⟧ e). *)
+
+Definition subtyping (Γ: listctx rty) (ρ1 ρ2: rty) : Prop :=
+      (* Assume [ρ1] and [ρ2] are valid [rty]s. *)
+      ⌊ ρ1 ⌋ = ⌊ ρ2 ⌋ /\ 
+      (is_coverage_rty ρ1 <-> is_coverage_rty ρ2) /\
+        forall (σ2: env), ⟦ Γ ⟧ σ2 ->
+        exists (σ1: env), ⟦ Γ ⟧ σ1 /\ 
+        [D ctxOverBindings Γ ∪ stale ρ2 ] σ1 = [D ctxOverBindings Γ ∪ stale ρ2 ] σ2 /\
+          (forall (e: tm), ⟦m{ σ1 } ρ1⟧ e -> ⟦m{ σ2 } ρ2⟧ e).
 
 Notation " Γ '⊢' τ1 '<⋮' τ2 " := (subtyping Γ τ1 τ2) (at level 20, τ1 constr, τ2 constr, Γ constr).
 
 Definition join (Γ: listctx rty) (ρ1 ρ2 ρ3: rty) : Prop :=
   (* Assume [ρ1] and [ρ2] are valid [rty]s. *)
   ⌊ ρ1 ⌋ = ⌊ ρ2 ⌋ /\ ⌊ ρ1 ⌋ = ⌊ ρ3 ⌋ /\
-    (is_coverage_rty ρ1 <-> is_coverage_rty ρ2) /\ (is_coverage_rty ρ1 <-> is_coverage_rty ρ3) /\
-    forall epr, ctxRst Γ epr -> exists Γv, eprR epr Γv ->
-                            forall e, ⟦m{ Γv }r ρ3⟧ e <-> ⟦m{ Γv }r ρ1⟧ e \/ ⟦m{ Γv }r ρ2⟧ e.
-
-Notation " Γ '⊢' τ1 '<⋮' τ2 " := (subtyping Γ τ1 τ2) (at level 20, τ1 constr, τ2 constr, Γ constr).
+    (is_coverage_rty ρ1 <-> is_coverage_rty ρ2) /\ 
+    (is_coverage_rty ρ1 <-> is_coverage_rty ρ3) /\
+    forall (e: tm) (σ: env), ⟦ Γ ⟧ σ -> ⟦m{ σ } ρ3⟧ e <-> ⟦m{ σ } ρ1⟧ e /\ ⟦m{ σ } ρ2⟧ e.
 
 Notation " Γ '⊢' τ1 '⋮merge' τ2 '⋮=' τ3" := (join Γ τ1 τ2 τ3) (at level 20, τ1 constr, τ2 constr, τ3 constr, Γ constr).
 
 (* The builtin typing relation (Δ) that our type system is parameterized over. *)
 Parameter builtin_typing_relation : effop -> rty -> Prop.
 
-Reserved Notation "Γ '⊢' op '⋮o' ρ"  (at level 20).
-Reserved Notation "Γ '⊢' e '⋮t' τ" (at level 20).
-Reserved Notation "Γ '⊢' e '⋮v' τ" (at level 20).
+Class TypingRefinement G E T := has_refinement_type : G -> E -> T -> Prop.
+
+Notation "Γ '⊢r' e '⋮' T" := (has_refinement_type Γ e T) (at level 20, e constr, T constr, Γ constr).
 
 (** * Typing rules (Fig. 6) *)
 
@@ -77,101 +60,115 @@ Inductive effop_type_check : listctx rty -> effop -> rty -> Prop :=
 | TEOp : forall Γ op ρ_op ρ,
     Γ ⊢WF ρ ->
     builtin_typing_relation op ρ_op ->
+    stale ρ_op = ∅ ->
     (* [TSubEOp] is inlined here. Consecutive applications of subtyping is just
     one subtyping. *)
     Γ ⊢ ρ_op <⋮ ρ ->
     ⌊ ρ ⌋ = ty_of_op op ->
-    Γ ⊢ op ⋮o ρ
-where
-"Γ '⊢' op '⋮o' ρ" := (effop_type_check Γ op ρ).
+    Γ ⊢ op ⋮ ρ.
+
+#[global] Instance TypingRefinement_effop: TypingRefinement (listctx rty) effop rty := effop_type_check.
 
 (** Typing rules for values and terms. Values always have refinement types, while
   terms always have Hoare automata types. *)
 Inductive term_type_check : listctx rty -> tm -> rty -> Prop :=
-| TErr: forall Γ (b: base_ty), Γ ⊢WF (mk_bot b) -> Γ ⊢ (terr b) ⋮t (mk_bot b)
-| TValue: forall Γ v τ, Γ ⊢ v ⋮v τ -> Γ ⊢ (treturn v) ⋮t τ
-| TSub: forall Γ e (τ1 τ2: rty),
+| TErr: forall Γ (b: base_ty), 
+  Γ ⊢WF (mk_bot b) -> term_type_check Γ (terr b) (mk_bot b)
+| TValue: forall Γ v τ,
+  value_type_check Γ v τ -> Γ ⊢r (treturn v) ⋮ τ
+| TSub: forall Γ (e: tm) (τ1 τ2: rty),
     Γ ⊢WF τ2 ->
-    Γ ⊢ e ⋮t τ1 ->
-    Γ ⊢ τ1 <⋮ τ2 ->
-    Γ ⊢ e ⋮t τ2
+    term_type_check [] e τ1 ->
+    [] ⊢ τ1 <⋮ τ2 ->
+    term_type_check Γ e τ2
 | TMerge: forall Γ e (τ1 τ2 τ3: rty),
     Γ ⊢WF τ3 ->
-    Γ ⊢ e ⋮t τ1 ->
-    Γ ⊢ e ⋮t τ2 ->
+    term_type_check Γ e τ1 ->
+    term_type_check Γ e τ2 ->
     Γ ⊢ τ1 ⋮merge τ2 ⋮= τ3 ->
-    Γ ⊢ e ⋮t τ3
+    stale e ⊆ ctxOverBindings Γ ->
+    term_type_check Γ e τ3
 | TLetE: forall Γ e1 e2 τ1 τ2 (L: aset),
-    (forall x, x ∉ L -> (Γ ++ [(x, τ1)]) ⊢ (e2 ^t^ x) ⋮t τ2) ->
+    (forall x, x ∉ L -> term_type_check (Γ ++ [(x, τ1)]) (e2 ^^ (vfvar x)) τ2) ->
     Γ ⊢WF τ2 ->
-    Γ ⊢ e1 ⋮t τ1 ->
-    Γ ⊢ (tlete e1 e2) ⋮t τ2
+    term_type_check Γ e1 τ1 ->
+    term_type_check Γ (tlete e1 e2) τ2
 | TAppOverParam: forall Γ (v1 v2: value) e b ϕ τ1 τ2 (L: aset),
-    (forall x, x ∉ L -> (Γ ++ [(x, τ1 ^r^ v2)]) ⊢ (e ^t^ x) ⋮t τ2) ->
+    (forall x, x ∉ L -> 
+      term_type_check (Γ ++ [(x, τ1 ^^ v2)]) (e ^^ (vfvar x)) τ2) ->
     Γ ⊢WF τ2 ->
-    Γ ⊢ v2 ⋮v [:b | ϕ] ->
-    Γ ⊢ v1 ⋮v ({:b | ϕ} ⇨ τ1) ->
-    Γ ⊢ (tletapp v1 v2 e) ⋮t τ2
+    value_type_check Γ v2 [:b | ϕ] ->
+    value_type_check Γ v1 ({:b | ϕ} ⇨ τ1) ->
+    term_type_check Γ (tletapp v1 v2 e) τ2
 | TAppFuncParam: forall Γ (v1 v2: value) e ρ1 ρ2 τ1 τ2 (L: aset),
-    (forall x, x ∉ L -> (Γ ++ [(x, τ1 ^r^ v2)]) ⊢ (e ^t^ x) ⋮t τ2) ->
+    (forall x, x ∉ L -> 
+      term_type_check (Γ ++ [(x, τ1 ^^ v2)]) (e ^^ (vfvar x)) τ2) ->
     Γ ⊢WF τ2 ->
-    Γ ⊢ v2 ⋮v (ρ1 ⇨ ρ2) ->
-    Γ ⊢ v1 ⋮v ((ρ1 ⇨ ρ2) ⇨ τ1) ->
-    Γ ⊢ (tletapp v1 v2 e) ⋮t τ2
+    value_type_check Γ v2 (ρ1 ⇨ ρ2) ->
+    value_type_check Γ v1 ((ρ1 ⇨ ρ2) ⇨ τ1) ->
+    term_type_check Γ (tletapp v1 v2 e) τ2
 | TAppOp: forall Γ (op: effop) (v2: value) e b ϕ b1 ϕ1 τ2 (L: aset),
-    (forall x, x ∉ L -> (Γ ++ [(x, [: b1 | ϕ1] ^r^ v2)]) ⊢ (e ^t^ x) ⋮t τ2) ->
+    (forall x, x ∉ L -> 
+      term_type_check (Γ ++ [(x, [: b1 | ϕ1] ^^ v2)]) (e ^^ (vfvar x)) τ2) ->
     Γ ⊢WF τ2 ->
-    Γ ⊢ v2 ⋮v [: b | ϕ] ->
-    Γ ⊢ op ⋮o ({: b | ϕ} ⇨ [: b1 | ϕ1]) ->
-    Γ ⊢ (tleteffop op v2 e) ⋮t τ2
+    value_type_check Γ v2 [: b | ϕ] ->
+    Γ ⊢r op ⋮ ({: b | ϕ} ⇨ [: b1 | ϕ1]) ->
+    term_type_check Γ (tleteffop op v2 e) τ2
 | TMatchbTrue: forall Γ (v: value) e1 e2 ϕ τ (L : aset),
     Γ ⊢WF τ ->
-    Γ ⊢ v ⋮v [:TBool | ϕ] ->
-    (forall x, x ∉ L -> (Γ ++ [(x, [: TBool | b0:c=true & b0:v= v & ϕ])]) ⊢ e1 ⋮t τ) ->
-    Γ ⊢ (tmatchb v e1 e2) ⋮t τ
+    value_type_check Γ v [:TBool | ϕ] ->
+    ⌊ Γ ⌋* ⊢ e2 ⋮ ⌊τ⌋ ->
+    (forall x, x ∉ L -> 
+      term_type_check (Γ ++ [(x, [: TBool | b0:c=true & b0:v= v & ϕ])]) e1 τ) ->
+    term_type_check Γ (tmatchb v e1 e2) τ
 | TMatchbFalse: forall Γ (v: value) e1 e2 ϕ τ (L : aset),
     Γ ⊢WF τ ->
-    Γ ⊢ v ⋮v [:TBool | ϕ] ->
-    (forall x, x ∉ L -> (Γ ++ [(x, [: TBool | b0:c=false & b0:v= v & ϕ])]) ⊢ e2 ⋮t τ) ->
-    Γ ⊢ (tmatchb v e1 e2) ⋮t τ
+    value_type_check Γ v [:TBool | ϕ] ->
+    ⌊ Γ ⌋* ⊢ e1 ⋮ ⌊τ⌋ ->
+    (forall x, x ∉ L -> 
+      term_type_check (Γ ++ [(x, [: TBool | b0:c=false & b0:v= v & ϕ])]) e2 τ) ->
+    term_type_check Γ (tmatchb v e1 e2) τ
 with value_type_check : listctx rty -> value -> rty -> Prop :=
 | TSubPP: forall Γ (v: value) (ρ1 ρ2: rty),
     Γ ⊢WF ρ2 ->
-    Γ ⊢ v ⋮v ρ1 ->
-    Γ ⊢ ρ1 <⋮ ρ2 ->
-    Γ ⊢ v ⋮v ρ2
+    value_type_check [] v ρ1 ->
+    [] ⊢ ρ1 <⋮ ρ2 ->
+    value_type_check Γ v ρ2
 | TConst: forall Γ (c: constant),
     Γ ⊢WF (mk_eq_constant c) ->
-    Γ ⊢ c ⋮v (mk_eq_constant c)
+    value_type_check Γ (vconst c) (mk_eq_constant c)
 | TBaseVar: forall Γ (x: atom) b ϕ,
     Γ ⊢WF (mk_eq_var b x) ->
     ctxfind Γ x = Some {: b | ϕ} ->
-    Γ ⊢ x ⋮v (mk_eq_var b x)
+    value_type_check Γ (vfvar x) (mk_eq_var b x)
 | TFuncVar: forall Γ (x: atom) ρ τ,
     Γ ⊢WF (ρ ⇨ τ) ->
     ctxfind Γ x = Some (ρ ⇨ τ) ->
-    Γ ⊢ x ⋮v (ρ ⇨ τ)
+    value_type_check Γ (vfvar x) (ρ ⇨ τ)
 | TFun: forall Γ Tx ρ e τ (L: aset),
     Γ ⊢WF (ρ ⇨ τ) ->
-    (forall x, x ∉ L -> (Γ ++ [(x, ρ)]) ⊢ (e ^t^ x) ⋮t (τ ^r^ x)) ->
+    (forall x, x ∉ L -> 
+      term_type_check (Γ ++ [(x, ρ)]) (e ^^ (vfvar x)) (τ ^^ (vfvar x))) ->
     Tx = ⌊ ρ ⌋ ->
-    Γ ⊢ (vlam Tx e) ⋮v (ρ ⇨ τ)
+    value_type_check Γ (vlam Tx e) (ρ ⇨ τ)
 | TFix: forall Γ (Tx : base_ty) ϕ e τ T (L: aset),
     Γ ⊢WF ({: Tx | ϕ} ⇨ τ) ->
     (* NOTE: should not open the whole type, because the first argument (bound *)
 (*     variable 0) of the return type is not the fixed point function but [{: Tx | *)
 (*     ϕ}]. The return type should be opened by [x]. *)
     (forall x, x ∉ L ->
-          (Γ ++ [(x, {: Tx | ϕ})]) ⊢ (vlam (Tx ⤍ T) e) ^v^ x ⋮v (({: Tx | b0:x≺ x & ϕ} ⇨ τ) ⇨ (τ ^r^ x))) ->
+          value_type_check (Γ ++ [(x, {: Tx | ϕ})]) ((vlam (Tx ⤍ T) e) ^^ (vfvar x)) (({: Tx | b0:x≺ x & ϕ} ⇨ τ) ⇨ (τ ^^ (vfvar x)))) ->
     T = ⌊ τ ⌋ ->
-    Γ ⊢ (vfix (Tx ⤍ T) (vlam (Tx ⤍ T) e)) ⋮v ({: Tx | ϕ} ⇨ τ)
-where
-"Γ '⊢' e '⋮t' τ" := (term_type_check Γ e τ) and "Γ '⊢' e '⋮v' ρ" := (value_type_check Γ e ρ).
+    value_type_check Γ (vfix (Tx ⤍ T) (treturn (vlam (Tx ⤍ T) e))) ({: Tx | ϕ} ⇨ τ).
 
 Scheme value_term_type_check_ind := Minimality for value_type_check Sort Prop
     with term_value_type_check_ind := Minimality for term_type_check Sort Prop.
 Combined Scheme value_term_type_check_mutind from
   value_term_type_check_ind, term_value_type_check_ind.
+
+#[global] Instance TypingRefinement_value: TypingRefinement (listctx rty) value rty := value_type_check.
+
+#[global] Instance TypingRefinement_tm: TypingRefinement (listctx rty) tm rty := term_type_check.
 
 (** * Properties of the type system *)
 
@@ -197,25 +194,25 @@ Qed.
 
 
 Lemma effop_typing_preserves_basic_typing Γ ρ op :
-  Γ ⊢ op ⋮o ρ ->
+  Γ ⊢r op ⋮ ρ ->
   ⌊ρ⌋ = ty_of_op op.
 Proof.
   inversion 1; subst. eauto.
 Qed.
 
 Lemma value_typing_regular_wf : forall (Γ: listctx rty) (v: value) (ρ: rty),
-    Γ ⊢ v ⋮v ρ -> Γ ⊢WF ρ
+    Γ ⊢r v ⋮ ρ -> Γ ⊢WF ρ
 with tm_typing_regular_wf : forall (Γ: listctx rty) (e: tm) (τ: rty),
-    Γ ⊢ e ⋮t τ -> Γ ⊢WF τ.
+    Γ ⊢r e ⋮ τ -> Γ ⊢WF τ.
 Proof.
   all: destruct 1; eauto.
 Qed.
 
 Lemma value_tm_typing_regular_is_coverage_rty:
   (forall (Γ: listctx rty) (v: value) (ρ: rty),
-      Γ ⊢ v ⋮v ρ -> is_coverage_rty ρ) /\
+      Γ ⊢r v ⋮ ρ -> is_coverage_rty ρ) /\
     (forall (Γ: listctx rty) (e: tm) (τ: rty),
-        Γ ⊢ e ⋮t τ -> is_coverage_rty τ).
+        Γ ⊢r e ⋮ τ -> is_coverage_rty τ).
 Proof.
   split; intros.
   - apply value_typing_regular_wf in H; intuition.
@@ -224,12 +221,15 @@ Qed.
 
 Lemma value_tm_typing_regular_basic_typing:
   (forall (Γ: listctx rty) (v: value) (ρ: rty),
-    Γ ⊢ v ⋮v ρ -> ⌊ Γ ⌋* ⊢t v ⋮v ⌊ ρ ⌋) /\
+    Γ ⊢r v ⋮ ρ -> ⌊ Γ ⌋* ⊢ v ⋮ ⌊ ρ ⌋) /\
   (forall (Γ: listctx rty) (e: tm) (τ: rty),
-    Γ ⊢ e ⋮t τ -> ⌊ Γ ⌋* ⊢t e ⋮t ⌊ τ ⌋).
+    Γ ⊢r e ⋮ τ -> ⌊ Γ ⌋* ⊢ e ⋮ ⌊ τ ⌋).
 Proof.
   apply value_term_type_check_mutind; intros; cbn; subst; eauto.
-  - hauto using rty_subtyping_preserves_basic_typing.
+  - apply rty_subtyping_preserves_basic_typing in H2. rewrite H2 in *.
+    unfold erase_ctx in H1. simplify_map_eq.
+    basic_typing_solver.
+  - (* TConst *) econstructor.
   - (* TBaseVar *) econstructor. qauto using ctx_erase_lookup.
   - (* TFuncVar *) econstructor. qauto using ctx_erase_lookup.
   - (* TFun *) econstructor.
@@ -244,105 +244,86 @@ Proof.
     rewrite <- rty_erase_open_eq in H1.
     eauto.
   - hauto using subtyping_preserves_basic_typing.
-  - hauto using subtyping_preserves_basic_typing.
-(*   - destruct ρ1; simpl in *. *)
-(*     all: econstructor; eauto; *)
-(*       instantiate_atom_listctx; *)
-(*       rewrite ctx_erase_app_r in H0 by my_set_solver; eauto. *)
-(*   - destruct ρ1; simpl in *. *)
-(*     all: auto_exists_L; intros; repeat specialize_with x; *)
-(*         rewrite ctx_erase_app_r in H0 by my_set_solver; *)
-(*         simpl in H0; repeat rewrite <- rty_erase_open_eq in H0; eauto. *)
-(*   - apply effop_typing_preserves_basic_typing in H4. cbn in H4. sinvert H4. *)
-(*     econstructor; eauto. qauto. *)
-(*     instantiate_atom_listctx. *)
-(*     rewrite ctx_erase_app_r in H0 by my_set_solver. *)
-(*     rewrite <- rty_erase_open_eq in H0; eauto. *)
-(*   - auto_pose_fv x. repeat specialize_with x. *)
-(*     rewrite ctx_erase_app_r in H3, H5 by my_set_solver. *)
-(*     econstructor; eauto. *)
-(*     eapply basic_typing_strengthen_tm; eauto. my_set_solver. *)
-(*     eapply basic_typing_strengthen_tm; eauto. my_set_solver. *)
-(* Qed. *)
-Admitted.
-
-Lemma value_typing_regular_basic_typing: forall (Γ: listctx rty) (v: value) (ρ: rty),
-    Γ ⊢ v ⋮v ρ -> ⌊ Γ ⌋* ⊢t v ⋮v ⌊ ρ ⌋.
-Proof.
-  apply value_tm_typing_regular_basic_typing.
+  - econstructor. eauto. 
+  - apply rty_subtyping_preserves_basic_typing in H2. rewrite H2 in *.
+    unfold erase_ctx in H1. simplify_map_eq.
+    basic_typing_solver.
+  - (* TMerge *) unfold join in *. mydestr. hauto.
+  - (* TLetE *) econstructor; eauto.
+    instantiate_atom_listctx. fold_typing_class.
+    rewrite ctx_erase_app_r in H0 by my_set_solver. eauto.
+  - destruct τ1; simpl in *.
+    all: econstructor; eauto;
+      instantiate_atom_listctx;
+      rewrite ctx_erase_app_r in H0 by my_set_solver; eauto.
+    ln_simpl. repeat rewrite <- rty_erase_open_eq in H0. eauto.
+  - destruct τ1; simpl in *.
+  all: econstructor; eauto;
+    instantiate_atom_listctx;
+    rewrite ctx_erase_app_r in H0 by my_set_solver; eauto.
+  ln_simpl. repeat rewrite <- rty_erase_open_eq in H0. eauto.  
+  - apply effop_typing_preserves_basic_typing in H4.
+    cbn in H4. sinvert H4.
+    econstructor; eauto.
+    instantiate_atom_listctx.
+    rewrite ctx_erase_app_r in H0 by my_set_solver.
+    rewrite <- rty_erase_open_eq in H0; eauto.
+  - (* TMatchbTrue *) econstructor; eauto.
+    all: 
+    auto_pose_fv x; repeat specialize_with x;
+    rewrite ctx_erase_app_r in H4 by my_set_solver; ln_simpl;
+    eapply basic_typing_strengthen_tm; eauto; my_set_solver.
+  - (* TMatchbFalse *) econstructor; eauto.
+    all: 
+    auto_pose_fv x; repeat specialize_with x;
+    rewrite ctx_erase_app_r in H4 by my_set_solver; ln_simpl;
+    eapply basic_typing_strengthen_tm; eauto; my_set_solver.
 Qed.
 
-Lemma tm_typing_regular_basic_typing: forall (Γ: listctx rty) (e: tm) (τ: rty),
-    Γ ⊢ e ⋮t τ -> ⌊ Γ ⌋* ⊢t e ⋮t ⌊ τ ⌋.
+Class RefinementTypingRegularBasicTyping (E: Type) `{Typing tyctx E ty} `{TypingRefinement (listctx rty) E rty} := refinement_typing_regular_basic_typing: forall (Γ: listctx rty) (e: E) (T: rty), Γ ⊢r e ⋮ T -> ⌊ Γ ⌋* ⊢ e ⋮ ⌊ T ⌋.
+
+#[global] Instance RefinementTypingRegularBasicTyping_value: RefinementTypingRegularBasicTyping value.
 Proof.
-  apply value_tm_typing_regular_basic_typing.
+  unfold RefinementTypingRegularBasicTyping.
+  eapply value_tm_typing_regular_basic_typing; eauto.
 Qed.
 
-(* Lemma ctxRst_insert_easy Γ P (x: atom) ρ P': *)
-(*     ctxRst Γ P -> *)
-(*     x ∉ ctxdom Γ -> *)
-(*     (forall env (v: value), ⟦ m{ env }r ρ ⟧ v -> P env <-> P' (<[ x := v ]> env)) -> *)
-(*     ctxRst (Γ ++ [(x, ρ)]) P'. *)
-(* Proof. *)
-(*   intros. econstructor; eauto. *)
-(*   econstructor; eauto using ctxRst_ok_ctx. *)
-(*   apply rtyR_typed_closed in H1. simp_hyps. *)
-(*   (* This should be a lemma similar to [msubst_preserves_closed_rty_empty], or *)
-(*   we should strenghthen this lemma. But don't bother now as it is only used *)
-(*   here. *) *)
-(*   sinvert H3. *)
-(*   econstructor. eauto using lc_msubst_rty, ctxRst_lc. *)
-(*   rewrite fv_of_msubst_rty_closed in H5 by eauto using ctxRst_closed_env. *)
-(*   rewrite ctxRst_dom in * by eauto. *)
-(*   my_set_solver. *)
-(* Qed. *)
+#[global] Instance RefinementTypingRegularBasicTyping_tm: RefinementTypingRegularBasicTyping tm.
+Proof.
+  unfold RefinementTypingRegularBasicTyping.
+  eapply value_tm_typing_regular_basic_typing; eauto.
+Qed.
 
-(* Lemma ctxRst_ctxfind Γ Γv x ρ : *)
-(*   ctxRst Γ Γv -> *)
-(*   ctxfind Γ x = Some ρ -> *)
-(*   fine_rty ρ -> *)
-(*   exists (v : value), Γv !! x = Some v /\ ⟦ m{ Γv }r ρ ⟧ v. *)
-(* Proof. *)
-(*   induction 1. *)
-(*   - easy. *)
-(*   - intros. *)
-(*     select (ctxfind (_ ++ _) _ = _) *)
-(*       (fun H => apply ctxfind_app in H; eauto using ok_ctx_ok). *)
+Class RefinementTypingRegular (E: Type) 
+`{Stale E}
+`{Typing tyctx E ty} `{TypingRefinement (listctx rty) E rty} `{RefinementTypingRegularBasicTyping E} := refinement_typing_regular: forall (Γ: listctx rty) (e: E) (T: rty), Γ ⊢r e ⋮ T -> 
+⌊ Γ ⌋* ⊢ e ⋮ ⌊ T ⌋ /\ Γ ⊢WF T.
 
-(*     assert (forall (v' : value), (⟦(m{env}r) ρ⟧) v' -> *)
-(*                             (⟦(m{<[x0:=v]> env}r) ρ⟧) v'). { *)
-(*       select (⟦ _ ⟧ _) (fun H => apply rtyR_typed_closed in H). simp_hyps. *)
-(*       intros. *)
-(*       apply rtyR_msubst_insert_eq; eauto using ctxRst_closed_env. *)
-(*       select (_ ⊢t _ ⋮t _) *)
-(*         (fun H => apply basic_typing_contains_fv_tm in H; simpl in H). *)
-(*       my_set_solver. *)
-(*       select (ok_ctx _) (fun H => apply ok_ctx_ok in H; apply ok_post_destruct in H). *)
-(*       srewrite ctxRst_dom. *)
-(*       simp_hyps. *)
-(*       apply not_elem_of_dom. eauto. *)
-(*     } *)
-(*     destruct_or!; simp_hyps. *)
-(*     + eexists. split; eauto. *)
-(*       assert (x <> x0). { *)
-(*         select (ok_ctx _) (fun H => sinvert H); listctx_set_simpl. *)
-(*         select (ctxfind _ _ = _) (fun H => apply ctxfind_some_implies_in_dom in H). *)
-(*         my_set_solver. *)
-(*       } *)
-(*       by simplify_map_eq. *)
-(*     + simpl in *. *)
-(*       case_decide; try easy. simplify_eq. *)
-(*       eexists. split; eauto. by simplify_map_eq. *)
-(* Qed. *)
+#[global] Instance RefinementTypingRegular_value: RefinementTypingRegular value.
+Proof.
+  unfold RefinementTypingRegular.
+  split.
+  - apply refinement_typing_regular_basic_typing; eauto.
+  - apply value_typing_regular_wf in H; eauto.
+Qed.
 
-Ltac msubst_erase_simp :=
-  repeat match goal with
-    | [H: context [ ⌊ ?τ ⌋ ] |- _ ] =>
-        match τ with
-        | context [ m{_}r _ ] => setoid_rewrite <- rty_erase_msubst_eq in H
-        end
-    | [H: _ |- context [ ⌊ ?τ ⌋ ]] =>
-        match τ with
-        | context [ m{_}r _ ] => setoid_rewrite <- rty_erase_msubst_eq
-        end
-    end.
+#[global] Instance RefinementTypingRegular_tm: RefinementTypingRegular tm.
+Proof.
+  unfold RefinementTypingRegular.
+  split.
+  - apply refinement_typing_regular_basic_typing; eauto.
+  - apply tm_typing_regular_wf in H; eauto.
+Qed.
+
+(** Convert an event operator to a value:
+  [op] is [fun x => leteffop y = op x in y] *)
+Definition value_of_op op : value :=
+  vlam TNat (tleteffop op (vbvar 0) (treturn (vbvar 0))).
+
+(** Well-formed built-in operator typing context (Definition 4.7) *)
+(* We simply treat the event operator as a value. This is equivalent to the
+definition in the paper (if we expand the denotation of this value). *)
+Definition well_formed_builtin_typing :=
+  forall op ρ,
+    builtin_typing_relation op ρ ->
+    ⟦ ρ ⟧ (treturn (value_of_op op)).
