DenotationProp.v
@@ -1,41 +1,12 @@
 From stdpp Require Import mapset.
 From stdpp Require Import natmap.
 From Stdlib.Program Require Import Wf.
-From CT Require Import CoreLangProp.
+From CT Require Import Syntax Lc.
 From CT Require Import OperationalSemantics.
 From CT Require Import BasicTypingProp.
-From CT Require Import RefinementTypeProp.
-From CT Require Import InstantiationProp.
 From CT Require Import Denotation.
 
-Import Atom.
-Import CoreLang.
-Import Tactics.
-Import NamelessTactics.
-Import ListCtx.
-Import OperationalSemantics.
-Import BasicTyping.
-Import Qualifier.
-Import RefinementType.
-Import Instantiation.
-Import Denotation.
-
-Ltac rtyR_regular_simp :=
-  (repeat match goal with
-     (* | [H: ctxRst _ _ |- lc _ ] => apply ctxRst_regular in H; simp_hyp H *)
-     (* | [H: ctxRst _ _ |- closed_env _ ] => apply ctxRst_regular in H; simp_hyp H *)
-     (* | [H: ctxRst _ _ |- ok_ctx _ ] => apply ctxRst_regular in H; simp_hyp H; eauto *)
-     (* | [H: ctxRst _ _ |- _ ∉ _ ] => apply ctxRst_regular in H; simp_hyp H; eauto *)
-     (* | [H: ctxRst _ ?Γv |- map_Forall _ ?Γv] => apply ctxRst_lc in H; eauto *)
-     | [H: rtyR _ _ _ |- lc _ ] => apply rtyR_typed_closed in H; simp_hyp H
-     | [H: rtyR _ _ _ |- lc_rty _ ] => apply rtyR_typed_closed in H; simp_hyp H
-     | [H: rtyR _ _ _ |- closed_value _ ] => apply rtyR_closed_value in H; eauto; simp_hyp H
-     | [H: rtyR _ _ _ |- closed_tm _ ] => apply rtyR_closed_tm in H; eauto; simp_hyp H
-     | [H: rtyR _ _ _ |- _ ⊢t _ ⋮v _ ] => apply rtyR_typed_closed in H; simp_hyp H
-     | [H: rtyR _ _ _ |- _ ⊢t _ ⋮t _ ] => apply rtyR_typed_closed in H; simp_hyp H
-     | [H: closed_rty _ _ |- lc_rty _ ] => destruct H; eauto
-     | [H: _ ≡ _ |- _ ∉ _ ] => rewrite H in *
-     end); basic_typing_regular_simp.
+Import BaseDef Lang MyTactics Primitives OperationalSemantics BasicTyping Qualifier RefinementType Instantiation ListCtx List LangLc Lc QualifierLc Denotation.
 
 (* Ltac is_tm_rty_tac := *)
 (*   match goal with *)
@@ -51,45 +22,90 @@ Ltac rtyR_regular_simp :=
 Lemma rtyR_refine_aux n: forall τ e1 e2,
     rty_measure τ <= n ->
     is_coverage_rty τ ->
-    tm_refine e1 e2 ->
+    e1 ⊑{ ⌊ τ ⌋ } e2 ->
     rtyR n τ e1 ->
     rtyR n τ e2.
 Proof.
   induction n; intros τ e1 e2 Hm Hunder [Ht Hr] H; simpl in *;
     destruct τ; simpl in *; eauto; try easy.
-  qauto using basic_typing_tm_unique.
   intuition.
-  - qauto using basic_typing_tm_unique.
-  - destruct H2 as (v & Hv & Hvv); subst.
-    exists v. intuition.
-  (*   eapply IHn; eauto. *)
-  (*   + repeat rewrite_measure_irrelevant. *)
-  (*     rewrite <- open_preserves_rty_measure. lia. *)
-  (*   + is_tm_rty_tac. *)
-  (*   + simp_hyps. unique_basic_type. *)
-  (*     eapply tm_refine_mk_app; eauto. *)
-  (*     * split; eauto. *)
-  (*     * rtyR_regular_simp. *)
-  (*     * eapply mk_app_e_v_has_type; eauto. *)
-  (*       rtyR_regular_simp. basic_typing_solver. *)
-  (* - intuition. qauto using basic_typing_tm_unique. *)
-  (*   destruct τ; eauto. *)
-  (*   intros. edestruct H2 as (v & Hv & Hvv); eauto. *)
+  - mydestr. repeat split; my_set_solver.
 Qed.
 
 Lemma rtyR_refine: forall τ e1 e2,
     is_coverage_rty τ ->
-    tm_refine e1 e2 ->
+    e1 ⊑{ ⌊ τ ⌋ } e2 ->
     ⟦ τ ⟧ e1 ->
     ⟦ τ ⟧ e2.
 Proof.
-  pose rtyR_refine_aux. eauto.
+  intros τ e1 e2 Hunder Hrefine Hdenote.
+  eapply rtyR_refine_aux with (n := rty_measure τ); eauto.
 Qed.
 
-Lemma denot_const_overrty (c: constant):
-  forall (T: base_ty) ϕ,
-    closed_rty ∅ {:T|ϕ} -> ∅ ⊢t c ⋮t T -> denote_qualifier (ϕ ^q^ c) -> (⟦{:T|ϕ}⟧) c.
+Lemma denot_const_overrty (c: constant) (b: base_ty) ϕ:
+    (⟦{:b|ϕ}⟧) (treturn (vconst c)) <-> 
+    stale {:b|ϕ} = ∅ /\ lc {:b|ϕ} /\ ∅ ⊢ (vconst c) ⋮ (TBase b) /\ ⟦ϕ ^^ (vconst c)⟧.
 Proof.
-  intros.
-  split; [| split]; eauto.
+  split; intros.
+  - sinvert H. ln_simpl. simp_hyps. repeat split; eauto.
+    basic_typing_solver.
+  - simp_hyps. econstructor; eauto.
+    basic_typing_solver.
 Qed.
+
+(* Lemma ctxRst_insert_easy Γ P (x: atom) ρ P': *)
+(*     ctxRst Γ P -> *)
+(*     x ∉ ctxdom Γ -> *)
+(*     (forall env (v: value), ⟦ m{ env }r ρ ⟧ v -> P env <-> P' (<[ x := v ]> env)) -> *)
+(*     ctxRst (Γ ++ [(x, ρ)]) P'. *)
+(* Proof. *)
+(*   intros. econstructor; eauto. *)
+(*   econstructor; eauto using ctxRst_ok_ctx. *)
+(*   apply rtyR_typed_closed in H1. simp_hyps. *)
+(*   (* This should be a lemma similar to [msubst_preserves_closed_rty_empty], or *)
+(*   we should strenghthen this lemma. But don't bother now as it is only used *)
+(*   here. *) *)
+(*   sinvert H3. *)
+(*   econstructor. eauto using lc_msubst_rty, ctxRst_lc. *)
+(*   rewrite fv_of_msubst_rty_closed in H5 by eauto using ctxRst_closed_env. *)
+(*   rewrite ctxRst_dom in * by eauto. *)
+(*   my_set_solver. *)
+(* Qed. *)
+
+(* Lemma ctxRst_ctxfind Γ Γv x ρ : *)
+(*   ctxRst Γ Γv -> *)
+(*   ctxfind Γ x = Some ρ -> *)
+(*   fine_rty ρ -> *)
+(*   exists (v : value), Γv !! x = Some v /\ ⟦ m{ Γv }r ρ ⟧ v. *)
+(* Proof. *)
+(*   induction 1. *)
+(*   - easy. *)
+(*   - intros. *)
+(*     select (ctxfind (_ ++ _) _ = _) *)
+(*       (fun H => apply ctxfind_app in H; eauto using ok_ctx_ok). *)
+
+(*     assert (forall (v' : value), (⟦(m{env}r) ρ⟧) v' -> *)
+(*                             (⟦(m{<[x0:=v]> env}r) ρ⟧) v'). { *)
+(*       select (⟦ _ ⟧ _) (fun H => apply rtyR_typed_closed in H). simp_hyps. *)
+(*       intros. *)
+(*       apply rtyR_msubst_insert_eq; eauto using ctxRst_closed_env. *)
+(*       select (_ ⊢ _ ⋮ _) *)
+(*         (fun H => apply basic_typing_contains_fv_tm in H; simpl in H). *)
+(*       my_set_solver. *)
+(*       select (ok_ctx _) (fun H => apply ok_ctx_ok in H; apply ok_post_destruct in H). *)
+(*       srewrite ctxRst_dom. *)
+(*       simp_hyps. *)
+(*       apply not_elem_of_dom. eauto. *)
+(*     } *)
+(*     destruct_or!; simp_hyps. *)
+(*     + eexists. split; eauto. *)
+(*       assert (x <> x0). { *)
+(*         select (ok_ctx _) (fun H => sinvert H); listctx_set_simpl. *)
+(*         select (ctxfind _ _ = _) (fun H => apply ctxfind_some_implies_in_dom in H). *)
+(*         my_set_solver. *)
+(*       } *)
+(*       by simplify_map_eq. *)
+(*     + simpl in *. *)
+(*       case_decide; try easy. simplify_eq. *)
+(*       eexists. split; eauto. by simplify_map_eq. *)
+(* Qed. *)
