LocallyNameless/InstantiationLc.v
@@ -1,0 +1,779 @@
+From stdpp Require Import mapset.
+From CT Require Import Syntax.
+Import BaseDef MyTactics Primitives Lang Instantiation.
+From CT.LocallyNameless Require Import LangLc QualifierLc RtyLc.
+
+(** This file proves auxiliary lemmas about multi-substitution and provides handy tactics. *)
+
+Lemma closed_env_insert env x v :
+  env !! x = None ->
+  closed_env (<[x:=v]>env) ->
+  stale v = ∅ /\ closed_env env.
+Proof.
+  intro.
+  unfold closed_env.
+  rewrite map_Forall_insert; eauto.
+Qed.
+
+Ltac gen_closed_env :=
+  repeat
+    match goal with
+    | H : closed_env (<[?i:=_]> ?m), H' : ?m !! ?i = None |- _ =>
+        let H1 := fresh "H" in
+        let H2 := fresh "H" in
+        destruct (closed_env_insert _ _ _ H' H) as [H1 H2];
+        uniq_hyp H1; uniq_hyp H2
+    | H : closed_env ?m, H' : ?m !! _ = Some ?v |- _ =>
+        let T := fresh "H" in
+        assert (stale v = ∅) as T by eauto;
+        uniq_hyp T
+    end.
+
+Class MsubstInsert A `{Subst value A} := msubst_insert: forall (σ: env) (x: atom) (v_x: value) (e: A),
+    closed_env σ ->
+    stale v_x = ∅ ->
+    σ !! x = None ->
+    msubst (<[x:=v_x]> σ) e = subst x v_x (msubst σ e).
+
+Lemma MsubstInsert_all
+    (A : Type)
+    (staleA : Stale A)
+    (substA : Subst value A)
+    (subst_commuteA : @SubstCommute A staleA substA)
+    : @MsubstInsert A substA.
+Proof.
+  unfold MsubstInsert.
+  intros.
+  apply map_fold_insert_L; eauto.
+  intros.
+  assert (closed_env (<[x:=v_x]>σ)). {
+    apply map_Forall_insert; eauto.
+  }
+  gen_closed_env.
+  apply subst_commute; eauto; my_set_solver.
+Qed.
+
+#[global] Instance MsubstInsert_tm: MsubstInsert tm.
+Proof.
+  eapply MsubstInsert_all; typeclasses eauto.
+Qed.
+
+#[global] Instance MsubstInsert_value: MsubstInsert value.
+Proof.
+  eapply MsubstInsert_all; typeclasses eauto.
+Qed.
+
+#[global] Instance MsubstInsert_qualifier: MsubstInsert qualifier.
+Proof.
+  eapply MsubstInsert_all; typeclasses eauto.
+Qed.
+
+#[global] Instance MsubstInsert_rty: MsubstInsert rty.
+Proof.
+  eapply MsubstInsert_all; typeclasses eauto.
+Qed.
+
+Ltac fold_forward :=
+  repeat match goal with
+    | H : map_fold ?f ?x ?m = _ |- context [ map_fold ?f ?x ?m ] => setoid_rewrite H
+    | H : forall _ _ _ _, map_fold _ _ (<[?i:= _]> _) = _ ?i _ (map_fold _ _ _) |-
+                       context [map_fold _ _ (<[?i:= _]> _) ] =>
+        rewrite H
+    | H : forall _ _ _ _, map_fold _ _ (<[?i:= _]> _) = _ ?i _ (map_fold _ _ _), H': context [map_fold _ _ (<[?i:= _]> _) ] |- _ =>
+        rewrite H in H'
+    end; eauto.
+
+(* Ltac apply_msubst_ind :=
+    unfold msubst;
+    match goal with
+    | |- ?T =>
+        match T with
+        | context [map_fold ?a ?b ?m] =>
+            match eval pattern (map_fold a b m) in T with
+            | ?P _ =>
+                match eval pattern m in P with
+                | ?P _ =>
+                    (* let P := eval simpl in (fun r m => P m r) in *)
+                    let P := eval simpl in (fun m => P m (msubst m b)) in
+                      apply (fin_maps.map_fold_ind P); unfold msubst
+                end
+            end
+        end
+    end. *)
+
+Ltac apply_msubst_ind :=
+  intros_until (amap value);
+  lazymatch goal with
+  | |- forall σ : env, ?body =>
+      let P := constr:(fun σ : env => body) in
+      apply (fin_maps.map_fold_ind P)
+  end; unfold msubst.
+
+(* Ltac apply_msubst_ind :=
+intros *;
+  match goal with
+    | |- context [msubst ?m _] =>
+          generalize dependent m
+    end;
+  lazymatch goal with
+  | |- forall σ : env, ?body =>
+      let P := constr:(fun σ : env => body) in
+      idtac P;
+      apply (fin_maps.map_fold_ind P); intros *
+  end; unfold msubst. *)
+
+Ltac msubst_tac :=
+  apply_msubst_ind; intros; subst; simpl; eauto;
+  gen_closed_env; simp_hyps; subst; fold_forward.
+
+(* Ltac msubst_tac' :=
+  intros *; apply_msubst_ind; intros; subst; simpl; eauto;
+  gen_closed_env; simp_hyps; subst; fold_forward. *)
+
+Ltac fold_msubst := change (map_fold ?s ?e ?m) with (@msubst m _ e s) in *.
+
+Ltac rewrite_msubst_insert :=
+  cbn; fold_msubst; rewrite !msubst_insert;
+  eauto using subst_commute.
+
+Lemma rty_erase_msubst_eq ρ: forall σ,
+  erase_rty ρ = erase_rty (m{σ} ρ).
+Proof.
+  msubst_tac.
+  qauto using rty_erase_subst_eq.
+Qed.
+
+Ltac msubst_hyp_rewrite :=
+  match goal with
+  | H : (msubst ?f ?m ?x) = _ |-
+      context [(msubst ?f ?m ?x) ] =>
+      rewrite H
+  end.
+
+Lemma msubst_qualifier: forall ϕ σ,
+    closed_env σ ->
+    (m{σ}) ϕ =
+      match ϕ with
+      | qual vals prop =>
+          qual (vmap (fun v => m{σ} v) vals) prop
+      end.
+Proof.
+  msubst_tac.
+  - destruct ϕ. erewrite Vector.map_ext.
+    by rewrite Vector.map_id.
+    intros. simpl.
+    by rewrite map_fold_empty.
+  - destruct ϕ.
+    ln_simpl.
+    f_equal. rewrite Vector.map_map.
+    apply Vector.map_ext.
+    intros; rewrite_msubst_insert.
+Qed.
+
+Lemma msubst_qualifier_and q1 q2: forall σ,
+  closed_env σ ->
+  m{σ} (q1 & q2) = (m{σ} q1) & (m{σ} q2).
+Proof.
+  msubst_tac. apply qualifier_and_subst.
+Qed.
+
+Lemma msubst_constant (c: constant): forall σ, (m{σ}) (vconst c) = vconst c.
+Proof.
+  msubst_tac.
+Qed.
+
+Lemma msubst_bvar: forall n σ, (m{σ}) (vbvar n) = vbvar n.
+Proof.
+  msubst_tac.
+Qed.
+
+Ltac class_simpl := autounfold with class_simpl; simpl; simplify_map_eq.
+
+Lemma msubst_fvar: forall (x : atom) σ,
+    closed_env σ ->
+    (m{σ}) (vfvar x) = match σ !! x with
+                 | Some v => v
+                 | None => vfvar x
+                 end.
+Proof.
+  msubst_tac.
+  destruct (decide (x = i)); subst; simplify_map_eq.
+  + class_simpl. reflexivity.
+  + case_match.
+    - apply subst_fresh. gen_closed_env. my_set_solver.
+    - class_simpl; eauto.
+Qed.
+
+Lemma msubst_lam: forall T e σ,
+    closed_env σ ->
+    ((m{σ}) (vlam T e)) = (vlam T ((m{σ}) e)).
+Proof.
+  msubst_tac.
+Qed.
+
+Lemma msubst_fix: forall T e σ,
+    closed_env σ ->
+    ((m{σ}) (vfix T e)) = (vfix T ((m{σ}) e)).
+Proof.
+  msubst_tac.
+Qed.
+
+Lemma msubst_value: forall (v:value) σ,
+    closed_env σ -> (m{σ}) (treturn v) = treturn ((m{σ}) v).
+Proof.
+  msubst_tac.
+Qed.
+
+Lemma msubst_err: forall (v:ty) σ,
+    closed_env σ -> (m{σ}) (terr v) = terr v.
+Proof.
+  msubst_tac.
+Qed.
+
+Lemma msubst_match: forall (v: value) e1 e2 σ,
+    closed_env σ ->
+    ((m{σ}) (tmatchb v e1 e2)) = tmatchb (m{σ} v) (m{σ} e1) (m{σ} e2).
+Proof.
+  msubst_tac.
+Qed.
+
+Lemma msubst_lete: forall e_x e (σ: env),
+    closed_env σ ->
+    (m{σ} (tlete e_x e) = tlete ((m{σ}) e_x) ((m{σ}) e)).
+Proof.
+  msubst_tac.
+Qed.
+
+Lemma msubst_tleteffop: forall op (v2: value) e σ,
+    closed_env σ ->
+    (m{σ}) (tleteffop op v2 e) = (tleteffop op (m{σ} v2) (m{σ} e)).
+Proof.
+  msubst_tac.
+Qed.
+
+Lemma msubst_tletapp: forall (v1 v2: value) e σ,
+    closed_env σ ->
+    (m{σ}) (tletapp v1 v2 e) = (tletapp (m{σ} v1) (m{σ} v2) (m{σ} e)).
+Proof.
+  msubst_tac.
+Qed.
+
+Lemma msubst_overrty: forall b ϕ σ,
+    closed_env σ ->
+    (m{σ}) {:b|ϕ} = {:b| (m{σ}) ϕ}.
+Proof.
+  msubst_tac.
+Qed.
+
+Lemma msubst_underrty: forall b ϕ σ,
+    closed_env σ ->
+    ((m{σ}) ([:b|ϕ])) = ([:b|(m{σ}) ϕ]).
+Proof.
+  msubst_tac.
+Qed.
+
+Lemma msubst_arrrty: forall ρ τ σ,
+    closed_env σ ->
+    ((m{σ}) (ρ⇨τ)) = ((m{σ} ρ)⇨(m{σ} τ)).
+Proof.
+  msubst_tac.
+Qed.
+
+Lemma msubst_flip_rty: forall (τ: rty) σ,
+    closed_env σ ->
+    m{σ} (flip_rty τ) = flip_rty (m{σ} τ).
+Proof.
+  destruct τ; simpl flip_rty; intros; eauto.
+  - rewrite msubst_overrty by eauto.
+    rewrite msubst_underrty; eauto.
+  - rewrite msubst_overrty by eauto.
+    rewrite msubst_underrty; eauto.
+  - repeat rewrite msubst_arrrty; eauto.
+Qed.
+
+(* Tactic Notation "rewrite_msubst" constr(lem) "in" hyp(H) := *)
+(*   rewrite lem in H; eauto using ctxEnv_closed_env. *)
+
+(* Tactic Notation "rewrite_msubst" constr(lem) := *)
+(*   rewrite lem in *; eauto using ctxEnv_closed_env. *)
+
+Class MsubstFresh (A: Type) `{Stale A} `{Subst value A} := msubst_fresh: forall (σ: env) (e: A),
+    stale σ ∩ stale e = ∅ ->
+    (m{σ}) e = e.
+
+Lemma MsubstFresh_all
+  (A : Type)
+  (staleA : Stale A)
+  (substA : Subst value A)
+  (subst_freshA : @SubstFresh A staleA substA)
+  : @MsubstFresh A staleA substA.
+Proof.
+  unfold MsubstFresh.
+  msubst_tac.
+  setoid_rewrite H1.
+  + rewrite subst_freshA; eauto.
+    ln_simpl. my_set_solver.
+  + ln_simpl. my_set_solver. 
+Qed.
+
+#[global] Instance MsubstFresh_tm: MsubstFresh tm.
+Proof.
+  eapply MsubstFresh_all; typeclasses eauto.
+Qed.
+
+#[global] Instance MsubstFresh_value: MsubstFresh value.
+Proof.
+  eapply MsubstFresh_all; typeclasses eauto.
+Qed.
+
+#[global] Instance MsubstFresh_qualifier: MsubstFresh qualifier.
+Proof.
+  eapply MsubstFresh_all; typeclasses eauto.
+Qed.
+
+#[global] Instance MsubstFresh_rty: MsubstFresh rty.
+Proof.
+  eapply MsubstFresh_all; typeclasses eauto.
+Qed.
+
+Lemma msubst_mk_top: forall (σ: env) b,
+    closed_env σ ->
+    m{σ} (mk_top b) = mk_top b.
+Proof.
+  intros.
+  rewrite msubst_fresh; eauto.
+  unfold mk_top, mk_q_under_top. ln_simpl. my_set_solver.
+Qed.
+
+Lemma msubst_mk_eq_constant: forall (σ: env) c,
+    closed_env σ ->
+    (m{σ}) (mk_eq_constant c) = (mk_eq_constant c).
+Proof.
+  intros.
+  rewrite msubst_fresh; eauto.
+  unfold mk_eq_constant, mk_q_bvar_eq_val.
+  ln_simpl. my_set_solver.
+Qed.
+
+Lemma msubst_mk_eq_var: forall (σ: env) b x v,
+    closed_env σ ->
+    σ !! x = Some v ->
+    (m{σ}) (mk_eq_var b x) = [:b | b0:v= v].
+Proof.
+  intros.
+  unfold mk_eq_var; eauto.
+  repeat rewrite msubst_underrty; eauto.
+  repeat rewrite msubst_qualifier; eauto.
+  simpl.
+  repeat rewrite msubst_bvar; eauto.
+  repeat rewrite msubst_fvar; eauto.
+  rewrite H0.
+  eauto.
+Qed.
+
+Lemma msubst_empty {A: Type} `{Subst value A} : forall (e: A), m{∅} e = e.
+Proof.
+  intros. unfold msubst.
+  rewrite map_fold_empty. auto.
+Qed.
+
+Ltac msubst_simp :=
+  match goal with
+  | |- context [ m{∅} _ ] => rewrite msubst_empty
+  | H: context [ m{∅} _ ] |- _ => rewrite msubst_empty in H
+  | H: context [ m{ _ } (tlete _ _) ] |- _ => rewrite msubst_lete in H
+  | |- context [ m{ _ } (tlete _ _) ] => rewrite msubst_lete
+  | H: context [ m{ _ } (tleteffop _ _ _) ] |- _ => rewrite msubst_tleteffop in H
+  | |- context [ m{ _ } (tleteffop _ _ _) ] => rewrite msubst_tleteffop
+  | H: context [ m{ _ } (tletapp _ _ _) ] |- _ => rewrite msubst_tletapp in H
+  | |- context [ m{ _ } (tletapp _ _ _) ] => rewrite msubst_tletapp
+  | H: context [ m{ _ } (vfix _ _) ] |- _ => rewrite msubst_fix in H
+  | |- context [ m{ _ } (vfix _ _) ] => rewrite msubst_fix
+  | H: context [ m{ _ } (treturn _) ] |- _ => rewrite msubst_value in H
+  | |- context [ m{ _ } (treturn _) ] => rewrite msubst_value
+  | H: context [ m{ _ } (vlam _ _) ] |- _ => rewrite msubst_lam in H
+  | |- context [ m{ _ } (vlam _ _) ] => rewrite msubst_lam
+  | H: context [ m{ _ } (terr _) ] |- _ => rewrite msubst_err in H
+  | |- context [ m{ _ } (terr _) ] => rewrite msubst_err
+  | H: context [ m{ _ } (tmatchb _ _ _) ] |- _ => rewrite msubst_match in H
+  | |- context [ m{ _ } (tmatchb _ _ _) ] => rewrite msubst_match
+  | H: context [ m{ _ } (vbvar _) ] |- _ => rewrite msubst_bvar in H
+  | |- context [ m{ _ } (vbvar _) ] => rewrite msubst_bvar
+  | H: context [ m{ _ } (vfvar _) ] |- _ => rewrite msubst_fvar in H
+  | |- context [ m{ _ } (vfvar _) ] => rewrite msubst_fvar
+  | H: context [ m{ _ } (vconst _) ] |- _ => rewrite msubst_constant in H
+  | |- context [ m{ _ } (vconst _) ] => rewrite msubst_constant
+  (* NOTE: don't unfold qualifier definition *)
+  (* | H: context [ m{ _ } _ ] |- _ => rewrite msubst_qualifier in H *)
+  (* | |- context [ m{ _ } _ ] => rewrite msubst_qualifier *)
+  | H: context [ m{ _ } (_ & _) ] |- _ => rewrite msubst_qualifier_and in H
+  | |- context [ m{ _ } (_ & _) ] => rewrite msubst_qualifier_and
+  | H: context [ m{ _ } {: _ | _ } ] |- _ => rewrite msubst_overrty in H
+  | |- context [ m{ _ } {: _ | _ } ] => rewrite msubst_overrty
+  | H: context [ m{ _ } [: _ | _ ] ] |- _ => rewrite msubst_underrty in H
+  | |- context [ m{ _ } [: _ | _ ] ] => rewrite msubst_underrty
+  | H: context [ m{ _ } (_ ⇨ _) ] |- _ => rewrite msubst_arrrty in H
+  | |- context [ m{ _ } (_ ⇨ _ ) ] => rewrite msubst_arrrty
+  | H: context [ m{ _ } (mk_top _) ] |- _ => rewrite msubst_mk_top in H
+  | |- context [ m{ _ } (mk_top _) ] => rewrite msubst_mk_top
+  | H: context [ m{ _ } (mk_eq_constant _) ] |- _ => rewrite msubst_mk_eq_constant in H
+  | |- context [ m{ _ } (mk_eq_constant _) ] => rewrite msubst_mk_eq_constant
+  | H: context [ m{ _ } (flip_rty _) ] |- _ => rewrite msubst_flip_rty in H
+  | |- context [ m{ _ } (flip_rty _) ] => rewrite msubst_flip_rty
+  | H: context [ m{ _ } (mk_eq_var _ ?x) ], H': _ !! ?x = Some ?v |- _ => rewrite msubst_mk_eq_var with (v:=v) in H
+  | H': _ !! ?x = Some ?v |- context [ m{ _ } (mk_eq_var _ ?x) ] => rewrite msubst_mk_eq_var with (v:=v)
+  end; eauto.
+
+(* Most lemmas here are generalization of the corresponding lemmas about
+single-substitution. *)
+
+Class MsubstOpenVar A `{Stale A} `{Open value A} `{Subst value A} `{Lc A} := msubst_open_var :
+forall e k (x: atom) (σ: env),
+    closed_env σ ->
+    map_Forall (fun _ v => lc (treturn v)) σ ->
+    x ∉ dom σ ->
+    (m{σ}) ({k ~> (vfvar x)} e) = {k ~> (vfvar x)} ((m{σ}) e).
+
+Lemma MsubstOpenVar_all
+(A : Type)
+(staleA : Stale A)
+(openA : Open value A)
+(substA : Subst value A)
+(lcA : Lc A)
+(* (subst_openA : @SubstOpenVar A staleA openA substA lcA) *)
+(subst_open_varA : @SubstOpenVar A staleA openA substA lcA)
+: @MsubstOpenVar A staleA openA substA lcA.
+Proof.
+  unfold MsubstOpenVar.
+  msubst_tac.
+  apply map_Forall_insert in H3; eauto.
+    setoid_rewrite H7; eauto.
+    apply subst_open_var.
+    all: lc_solver1; my_set_solver.
+Qed.
+
+#[global] Instance MsubstOpenVar_tm: MsubstOpenVar tm.
+Proof.
+  eapply MsubstOpenVar_all; typeclasses eauto.
+Qed.
+
+#[global] Instance MsubstOpenVar_value: MsubstOpenVar value.
+Proof.
+  eapply MsubstOpenVar_all; typeclasses eauto.
+Qed.
+
+#[global] Instance MsubstOpenVar_rty: MsubstOpenVar rty.
+Proof.
+  eapply MsubstOpenVar_all; typeclasses eauto.
+Qed.
+
+#[global] Instance MsubstOpenVar_qualifier: MsubstOpenVar qualifier.
+Proof.
+  eapply MsubstOpenVar_all; typeclasses eauto.
+Qed.
+
+Class MsubstOpen A `{Stale A} `{Open value A} `{Subst value A}  `{Lc A} := msubst_open :
+forall (ρ: A) k (v_x: value) (σ: env),
+    closed_env σ ->
+    map_Forall (fun _ v => lc (treturn v)) σ ->
+    (m{σ}) ({k ~> v_x} ρ) = {k ~> (m{σ} v_x)} (m{σ} ρ).
+
+Lemma MsubstOpen_all
+(A : Type)
+(staleA : Stale A)
+(openA : Open value A)
+(substA : Subst value A)
+(lcA : Lc A)
+(subst_openA : @SubstOpen A staleA openA substA lcA)
+: @MsubstOpen A staleA openA substA lcA.
+Proof.
+  unfold MsubstOpen.
+  msubst_tac.
+  apply map_Forall_insert in H3; eauto. simp_hyps.
+  fold_forward.
+  rewrite subst_openA; auto. 
+  lc_solver1; my_set_solver.
+Qed.
+
+#[global] Instance MsubstOpen_tm: MsubstOpen tm.
+Proof.
+  apply MsubstOpen_all; typeclasses eauto.
+Qed.
+
+#[global] Instance MsubstOpen_value: MsubstOpen value.
+Proof.
+  eapply MsubstOpen_all; typeclasses eauto.
+Qed.
+
+#[global] Instance MsubstOpen_rty: MsubstOpen rty.
+Proof.
+  eapply MsubstOpen_all; typeclasses eauto.
+Qed.
+
+#[global] Instance MsubstOpen_qualifier: MsubstOpen qualifier.
+Proof.
+  eapply MsubstOpen_all; typeclasses eauto.
+Qed.
+
+Class MsubstFv A `{Stale A} `{Subst value A} := msubst_fv :
+forall (σ: env) (e: A),
+    closed_env σ ->
+    stale (m{σ} e) ⊆ stale e.
+
+Lemma MsubstFv_all
+(A : Type)
+(staleA : Stale A)
+(openA : Open value A)
+(substA : Subst value A)
+(fv_of_subst_closedA : @FvOfSubstClosed A staleA substA)
+: @MsubstFv A staleA substA.
+Proof.
+  unfold MsubstFv.
+  msubst_tac.
+  rewrite fv_of_subst_closedA; my_set_solver.
+Qed.
+
+#[global] Instance MsubstFv_tm: MsubstFv tm.
+Proof.
+  eapply MsubstFv_all; typeclasses eauto.
+Qed.
+
+#[global] Instance MsubstFv_value: MsubstFv value.
+Proof.
+  eapply MsubstFv_all; typeclasses eauto.
+Qed.
+
+#[global] Instance MsubstFv_qualifier: MsubstFv qualifier.
+Proof.
+  eapply MsubstFv_all; typeclasses eauto.
+Qed.
+
+#[global] Instance MsubstFv_rty: MsubstFv rty.
+Proof.
+  eapply MsubstFv_all; typeclasses eauto.
+Qed.
+
+Class MsubstIntro A `{Stale A} `{Open value A} `{Subst value A} `{Lc A} := msubst_intro :
+forall (e: A) k (v_x: value) (x: atom) (σ: env),
+    closed_env σ ->
+    stale v_x = ∅ ->
+    lc v_x ->
+    map_Forall (fun _ v => lc (treturn v)) σ ->
+    x ∉ dom σ ∪ stale e ->
+    {k ~> v_x} ((m{σ}) e) = (m{<[x:=v_x]> σ}) ({k ~> (vfvar x)} e).
+
+Lemma MsubstIntro_all
+(A : Type)
+(staleA : Stale A)
+(openA : Open value A)
+(substA : Subst value A)
+(lcA : Lc A)
+(msubst_openA : @MsubstOpen A staleA openA substA lcA)
+(subst_freshA : @SubstFresh A staleA substA)
+(msubst_insertA : @MsubstInsert A substA)
+(msubst_fvA : @MsubstFv A staleA substA)
+: @MsubstIntro A staleA openA substA lcA.
+Proof.
+  unfold MsubstIntro.
+  intros.
+  assert (stale σ ∩ stale x = ∅) by my_set_solver.
+  assert (σ !! x = None). {
+     apply not_elem_of_dom. my_set_solver.
+  }
+  rewrite msubst_openA; auto.
+  rewrite_msubst_insert.
+  f_equal.
+  - rewrite msubst_fresh; eauto. 
+    autounfold with class_simpl in *. hauto.
+  - rewrite subst_freshA; eauto.
+    assert (stale ((m{σ}) e) ⊆ stale e) by eauto using msubst_fvA. my_set_solver. 
+  - apply map_Forall_insert; eauto.
+  - apply map_Forall_insert; eauto.
+    intuition. lc_solver1; my_set_solver.
+Qed. 
+
+#[global] Instance MsubstIntro_tm: MsubstIntro tm.
+Proof.
+  eapply MsubstIntro_all; typeclasses eauto.
+Qed.
+
+#[global] Instance MsubstIntro_value: MsubstIntro value.
+Proof.
+  eapply MsubstIntro_all; typeclasses eauto.
+Qed.
+
+#[global] Instance MsubstIntro_qualifier: MsubstIntro qualifier.
+Proof.
+  eapply MsubstIntro_all; typeclasses eauto.
+Qed.
+
+#[global] Instance MsubstIntro_rty: MsubstIntro rty.
+Proof.
+  eapply MsubstIntro_all; typeclasses eauto.
+Qed.
+
+Class MsubstInsertFresh A `{Stale A} `{Subst value A} := msubst_insert_fresh :
+forall (e: A) (x: atom) (v_x: value) (σ: env),
+    closed_env σ ->
+    stale v_x = ∅ ->
+    x ∉ dom σ ∪ stale e ->
+    (m{<[x:=v_x]> σ}) e = (m{σ}) e.
+
+Lemma MsubstInsertFresh_all
+(A : Type)
+(staleA : Stale A)
+(substA : Subst value A)
+(subst_freshA : @SubstFresh A staleA substA)
+(msubst_insertA : @MsubstInsert A substA)
+(msubst_fvA : @MsubstFv A staleA substA)
+: @MsubstInsertFresh A staleA substA.
+Proof.
+  unfold MsubstInsertFresh.
+  intros. rewrite_msubst_insert.
+  - apply subst_freshA.
+    pose proof (msubst_fvA σ e H).
+    eapply not_elem_of_weaken; eauto. my_set_solver.
+  - apply not_elem_of_dom; my_set_solver.
+Qed.
+
+#[global] Instance MsubstInsertFresh_tm: MsubstInsertFresh tm.
+Proof.
+  eapply MsubstInsertFresh_all; typeclasses eauto.
+Qed.
+
+#[global] Instance MsubstInsertFresh_value: MsubstInsertFresh value.
+Proof.
+  eapply MsubstInsertFresh_all; typeclasses eauto.
+Qed.
+
+#[global] Instance MsubstInsertFresh_qualifier: MsubstInsertFresh qualifier.
+Proof.
+  eapply MsubstInsertFresh_all; typeclasses eauto.
+Qed.
+
+#[global] Instance MsubstInsertFresh_rty: MsubstInsertFresh rty.
+Proof.
+  eapply MsubstInsertFresh_all; typeclasses eauto.
+Qed.
+
+Class MsubstLc A `{Stale A} `{Subst value A} `{Lc A} := msubst_lc :
+forall (e: A) (σ: env),
+    lc e ->
+    map_Forall (fun _ v => lc (treturn v)) σ ->
+    lc (m{σ} e).
+
+Lemma MsubstLc_all
+(A : Type)
+(staleA : Stale A)
+(substA : Subst value A)
+(lcA : Lc A)
+(subst_lcA : @SubstLc A staleA substA lcA)
+: @MsubstLc A staleA substA lcA.
+Proof.
+  unfold MsubstLc.
+  msubst_tac.
+  apply map_Forall_insert in H3; eauto.
+  apply subst_lcA. hauto. lc_solver1; my_set_solver.
+Qed.
+
+#[global] Instance MsubstLc_tm: MsubstLc tm.
+Proof.
+  eapply MsubstLc_all; typeclasses eauto.
+Qed.
+
+#[global] Instance MsubstLc_value: MsubstLc value.
+Proof.
+  eapply MsubstLc_all; typeclasses eauto.
+Qed.
+
+#[global] Instance MsubstLc_qualifier: MsubstLc qualifier.
+Proof.
+  eapply MsubstLc_all; typeclasses eauto.
+Qed.
+
+#[global] Instance MsubstLc_rty: MsubstLc rty.
+Proof.
+  eapply MsubstLc_all; typeclasses eauto.
+Qed.
+
+Class LcMsubst A `{Stale A} `{Subst value A} `{Lc A} := lc_msubst :
+forall (e: A) (σ: env),
+    lc (m{σ} e) ->
+    map_Forall (fun _ v => lc (treturn v)) σ ->
+    lc e.
+
+Lemma LcMsubst_all
+(A : Type)
+(staleA : Stale A)
+(substA : Subst value A)
+(lcA : Lc A)
+(lc_substA : @LcSubst A staleA substA lcA)
+: @LcMsubst A staleA substA lcA.
+Proof.
+  unfold LcMsubst.
+  msubst_tac.
+  apply map_Forall_insert in H3; eauto. simp_hyps.
+  assert (lc x) by lc_solver1; my_set_solver.
+Qed.
+
+#[global] Instance LcMsubst_tm: LcMsubst tm.
+Proof.
+  eapply LcMsubst_all; typeclasses eauto.
+Qed.
+
+#[global] Instance LcMsubst_value: LcMsubst value.
+Proof.
+  eapply LcMsubst_all; typeclasses eauto.
+Qed.
+
+#[global] Instance LcMsubst_qualifier: LcMsubst qualifier.
+Proof.
+  eapply LcMsubst_all; typeclasses eauto.
+Qed.
+
+#[global] Instance LcMsubst_rty: LcMsubst rty.
+Proof.
+  eapply LcMsubst_all; typeclasses eauto.
+Qed.
+
+Class FvOfMsubstClosed A `{Stale A} `{Subst value A} := fv_of_msubst_closed :
+forall (e: A) (σ: env),
+    closed_env σ ->
+    stale (m{σ} e) = stale e ∖ stale σ.
+
+Lemma FvOfMsubstClosed_all
+(A : Type)
+(staleA : Stale A)
+(substA : Subst value A)
+(fv_of_subst_closedA : @FvOfSubstClosed A staleA substA)
+: @FvOfMsubstClosed A staleA substA.
+Proof.
+  unfold FvOfMsubstClosed.
+  msubst_tac.
+  - rewrite map_fold_empty. my_set_solver.
+  - rewrite fv_of_subst_closedA.
+    + setoid_rewrite H5. ln_simpl.
+      autounfold with class_simpl. 
+      rewrite dom_insert_L. my_set_solver.
+    + hauto.
+Qed.
+
+#[global] Instance FvOfMsubstClosed_tm: FvOfMsubstClosed tm.
+Proof.
+  eapply FvOfMsubstClosed_all; typeclasses eauto.
+Qed.
+
+#[global] Instance FvOfMsubstClosed_value: FvOfMsubstClosed value.
+Proof.
+  eapply FvOfMsubstClosed_all; typeclasses eauto.
+Qed.
+
+#[global] Instance FvOfMsubstClosed_qualifier: FvOfMsubstClosed qualifier.
+Proof.
+  eapply FvOfMsubstClosed_all; typeclasses eauto.
+Qed.
+
+#[global] Instance FvOfMsubstClosed_rty: FvOfMsubstClosed rty.
+Proof.
+  eapply FvOfMsubstClosed_all; typeclasses eauto.
+Qed.
