World.v
@@ -1,0 +1,144 @@
+From stdpp Require Import mapset.
+From CT Require Import Syntax.
+From CT Require Import OperationalSemantics.
+From CT Require Import BasicTypingProp.
+
+Import BaseDef MyTactics Primitives Lang LangLc Qualifier OperationalSemantics BasicTyping BasicTypingProp.
+
+(** This file defines valuation environment, i.e., substitution (σ), and
+  multi-substitution operation. *)
+
+(** Environment (substitution) *)
+Notation env := (amap value).
+(** A world is a set of substitutions that satisfies a proposition.
+    π ⊧ P iff ∀ σ ∈ π, σ ⊧ P.
+    If π ⊧ P and P -> Q, then π ⊧ Q.
+    A world can also be treated as an abstraction of a set of propositions P (closed under implication).
+    The denotation of a type context is the set of propositions that are satisfied under the type context—a set of worlds (not a single world, because it may not be closed under implication).
+    ⟦Γ⟧ := { π | Γ ⊧ P ∧ π ⊧ P }
+    Γ ⊧ P iff there exists a world π in ⟦Γ⟧.
+    Assume mkWorld(P) is the minimal set of substitutions that satisfies P.
+    mkWorld(P) := {σ ∈ E | σ ⊧ P}
+    ⟦Γ⟧ := { mkWorld(P) | Γ ⊧ P }, closed with respect to the subset relation.
+    For example, mkWorld(x = y) :=
+      {[x := True, y := True], [x := False, y := False]}
+    For a world π = {[x := True, y := True]}, π ⊧ x = y.
+    For a type context x:{bool | v = True}, y:{bool | top },
+    its denotation contains all worlds including 
+    [x := True, y := True] and [x := True, y := False].
+    ⟦Γ⟧ = {
+      {[x := True, y := True], [x := True, y := False]}, 
+      {[x := True, y := True], [x := True, y := False], [x := False, y := False]},
+      ..., 
+    }
+    This means that it is free to pick any world from the denotation; if the world can entail the proposition P, it is sufficient to prove the proposition P.
+    For a type context x:{bool | v = True}, y:[bool | top ],
+    its denotation contains all worlds including 
+    [x := True, y := True] or [x := True, y := False].
+    ⟦Γ⟧ = {
+      {[x := True, y := True]}, 
+      {[x := True, y := False]},
+      {[x := True, y := False], [x := False, y := False]},
+      ..., 
+    }
+    For a type context x:[bool | top], y:[bool | v = x ],
+    its denotation contains all worlds including 
+    [x := True, y := True] or [x := False, y := False].
+    For a type context x:{bool | top}, y:[bool | v = x ],
+    its denotation contains all worlds including 
+    [x := True, y := True] and [x := False, y := False].
+*)
+Inductive world : Type :=
+| World (L: aset) (π: env -> Prop).
+(* Technically, we require the domain of all substitutions in the world to be the same (i.e., L). *)
+
+Definition closed_env (env : env) := map_Forall (fun _ v => stale v ≡ ∅) env.
+
+Inductive closed_world: world -> Prop :=
+| ClosedWorld: forall L π,
+    (forall σ, π σ -> dom σ ≡ L /\ closed_env σ) ->
+    closed_world (World L π).
+
+#[global] Instance world_stale : Stale world := 
+  fun w => match w with
+  | World L π => L
+  end.
+Arguments world_stale /.
+
+Definition emp_world : world := World ∅ (fun σ => σ = ∅).
+
+Lemma emp_world_closed: closed_world emp_world.
+Proof.
+  econstructor; eauto. split; eauto. my_set_solver. subst.
+  apply map_Forall_empty.
+Qed.
+
+Global Hint Resolve emp_world_closed: core.
+
+(* x is not in L *)
+Definition world_insert (x: atom) (vset: env -> value -> Prop) (w: world): world :=
+  match w with
+  | World L π => World (L ∪ {[x]}) 
+    (fun σ' => exists σ v, σ' = <[x:=v]> σ /\ π σ /\ vset σ v)
+  end.
+
+Lemma world_insert_stale x vset w :
+  stale (world_insert x vset w) = stale w ∪ {[x]}.
+Proof.
+  destruct w. ln_simpl; eauto.
+Qed.
+
+Definition world_models (w: world) (P: env -> Prop) :=
+  match w with
+  | World L π => forall σ, π σ -> P σ
+  end.
+  
+Notation "w '⊨' P " := (world_models w P) (at level 20, format "w ⊨ P", w constr, P constr).
+
+Lemma closed_world_closed_env w: closed_world w -> w ⊨ (fun σ => closed_env σ).
+Proof.
+  intros H.
+  inversion H; subst; eauto.
+  simpl. hauto.
+Qed.
+
+Definition world_models_implies (w: world) (P Q: env -> Prop) :
+  w ⊨ P -> (forall σ, P σ -> Q σ) -> w ⊨ Q.
+Proof.
+  intros Hmodels Himplies.
+  destruct w. hauto.
+Qed.
+
+Definition world_models_iff (w: world) (P Q: env -> Prop) :
+w ⊨ (fun σ => P σ <-> Q σ) <-> (w ⊨ (fun σ => P σ -> Q σ)) /\ (w ⊨ (fun σ => Q σ -> P σ)).
+Proof.
+  split; intros; destruct w; hauto.
+Qed.
+
+Definition world_models_and (w: world) (P Q: env -> Prop) :
+  (w ⊨ P /\ w ⊨ Q) <-> w ⊨ (fun σ => P σ /\ Q σ).
+Proof.
+  split; intros.
+  - mydestr. destruct w. hauto.
+  - destruct w. hauto. 
+Qed.
+
+Definition world_join (w1 w2: world) : world :=
+  match w1, w2 with
+  | World L1 π1, World L2 π2 => World (L1 ∪ L2) (fun σ => π1 σ \/ π2 σ)
+  end.
+
+Lemma world_join_models_left w1 w2 (P: env -> Prop):
+  w1 ⊨ (fun σ => P σ) -> (world_join w1 w2) ⊨ (fun σ => P σ).
+Proof.
+  intros Hmodels1; destruct w1, w2; simpl in *; eauto.
+  intros σ Hπ. apply Hmodels1 in Hπ. apply H. apply Hπ.
+  destruct w1, w2. hauto.
+Qed.
+
+(** Multi-substitution, i.e., σ(⋅) operation. The definition is parameterized by
+  any substitution. *)
+Definition msubst (env : env) {A: Type} (a : A) `{Subst value A} : A :=
+  map_fold subst a env.
+
+Notation "'m{' x '}'" := (msubst x) (at level 20, format "m{ x }", x constr).
